Added another file "Library/frag.ml" with a type constructor for defining the free Abelian group on a given type. Incorporated this into the general group theory. In that "Library/grouptheory.ml" file, systematically adopted a multiplicative terminology (changing various names from "op/OP" to "mul/MUL") as well as adding new material: powers (natural number and integer), trivial homomorphisms, Abelian groups, cyclic groups and the group of integers. Renamed theorems:
        GROUP_INV_OP            --> GROUP_INV_MUL
        GROUP_OP                --> GROUP_MUL
        GROUP_OP_ASSOC          --> GROUP_MUL_ASSOC
        GROUP_OP_LCANCEL        --> GROUP_MUL_LCANCEL
        GROUP_OP_LID            --> GROUP_MUL_LID
        GROUP_OP_LINV           --> GROUP_MUL_LINV
        GROUP_OP_RCANCEL        --> GROUP_MUL_RCANCEL
        GROUP_OP_RID            --> GROUP_MUL_RID
        GROUP_OP_RINV           --> GROUP_MUL_RINV
        GROUP_SETOP             --> GROUP_SETMUL
        GROUP_SETOP_ASSOC       --> GROUP_SETMUL_ASSOC
        GROUP_SETOP_EQ_EMPTY    --> GROUP_SETMUL_EQ_EMPTY
        GROUP_SETOP_LCANCEL     --> GROUP_SETMUL_LCANCEL
        GROUP_SETOP_LCANCEL_SET --> GROUP_SETMUL_LCANCEL_SET
        GROUP_SETOP_LEFT_COSET  --> GROUP_SETMUL_LEFT_COSET
        GROUP_SETOP_LID         --> GROUP_SETMUL_LID
        GROUP_SETOP_LSUBSET     --> GROUP_SETMUL_LSUBSET
        GROUP_SETOP_LSUBSET_EQ  --> GROUP_SETMUL_LSUBSET_EQ
        GROUP_SETOP_RCANCEL     --> GROUP_SETMUL_RCANCEL
        GROUP_SETOP_RCANCEL_SET --> GROUP_SETMUL_RCANCEL_SET
        GROUP_SETOP_RID         --> GROUP_SETMUL_RID
        GROUP_SETOP_RIGHT_COSET --> GROUP_SETMUL_RIGHT_COSET
        GROUP_SETOP_RSUBSET     --> GROUP_SETMUL_RSUBSET
        GROUP_SETOP_RSUBSET_EQ  --> GROUP_SETMUL_RSUBSET_EQ
        GROUP_SETOP_SING        --> GROUP_SETMUL_SING
        GROUP_SETOP_SUBGROUP    --> GROUP_SETMUL_SUBGROUP
        OPPOSITE_GROUP_OP       --> OPPOSITE_GROUP_MUL
        OPPOSITE_GROUP_SETOP    --> OPPOSITE_GROUP_SETMUL
        QUOTIENT_GROUP_OP       --> QUOTIENT_GROUP_MUL
        SUBGROUP_SETOP_EQ       --> SUBGROUP_SETMUL_EQ
        group_op                --> group_mul
        group_setop             --> group_setmul

and really new definitions and theorems:

        ABELIAN_FREE_ABELIAN_GROUP
        ABELIAN_GROUP_EPIMORPHIC_IMAGE
        ABELIAN_GROUP_HOMOMORPHISM_GROUP_MUL
        ABELIAN_GROUP_MUL_AC
        ABELIAN_GROUP_NORMAL_SUBGROUP
        ABELIAN_GROUP_QUOTIENT_GROUP
        ABELIAN_OPPOSITE_GROUP
        ABELIAN_SINGLETON_GROUP
        ABELIAN_SUBGROUP_GENERATED
        CARRIER_SUBGROUP_GENERATED_BY_SING
        CYCLIC_GROUP
        CYCLIC_GROUP_EPIMORPHIC_IMAGE
        CYCLIC_GROUP_QUOTIENT_GROUP
        CYCLIC_IMP_ABELIAN_GROUP
        DEST_FRAG_0
        DEST_FRAG_ADD
        DEST_FRAG_CMUL
        DEST_FRAG_NEG
        DEST_FRAG_OF
        DEST_FRAG_SUB
        FINITE_CYCLIC_SUBGROUP
        FINITE_CYCLIC_SUBGROUP_ALT
        FINITE_FRAG_SUPPORT
        FRAG_ADD_EQ_0
        FRAG_CLOSURE_SUB_CMUL
        FRAG_CMUL_SUM
        FRAG_EQ
        FRAG_EXPANSION
        FRAG_EXTEND
        FRAG_EXTEND_0
        FRAG_EXTEND_ADD
        FRAG_EXTEND_CMUL
        FRAG_EXTEND_COMPOSE
        FRAG_EXTEND_EQ
        FRAG_EXTEND_EQ_0
        FRAG_EXTEND_NEG
        FRAG_EXTEND_OF
        FRAG_EXTEND_SUB
        FRAG_EXTEND_SUM
        FRAG_INDUCTION
        FRAG_OF_NONZERO
        FRAG_SPLIT
        FRAG_SUPPORT_0
        FRAG_SUPPORT_ADD
        FRAG_SUPPORT_CMUL
        FRAG_SUPPORT_EQ_EMPTY
        FRAG_SUPPORT_FRAG_EXTEND
        FRAG_SUPPORT_NEG
        FRAG_SUPPORT_OF
        FRAG_SUPPORT_SUB
        FRAG_SUPPORT_SUM
        FREE_ABELIAN_GROUP
        GROUP_DIV_SUBGROUP_GENERATED
        GROUP_ENDOMORPHISM_INTEGER_GROUP_EQ
        GROUP_ENDOMORPHISM_INTEGER_GROUP_EQ_ALT
        GROUP_ENDOMORPHISM_INTEGER_GROUP_EXPLICIT
        GROUP_ENDOMORPHISM_INTEGER_GROUP_MUL
        GROUP_EPIMORPHISM_GROUP_ZPOW
        GROUP_EPIMORPHISM_TRIVIAL
        GROUP_HOMOMORPHISM_GROUP_ZPOW
        GROUP_HOMOMORPHISM_INV
        GROUP_HOMOMORPHISM_MUL
        GROUP_HOMOMORPHISM_POW
        GROUP_HOMOMORPHISM_TRIVIAL
        GROUP_HOMOMORPHISM_ZPOW
        GROUP_INV_POW
        GROUP_INV_ZPOW
        GROUP_ISOMORPHISM_GROUP_ZPOW
        GROUP_ISOMORPHISM_TRIVIAL
        GROUP_KERNEL_IMAGE_TRIVIAL
        GROUP_MONOMORPHISM_TRIVIAL
        GROUP_MUL_LCANCEL_IMP
        GROUP_MUL_RCANCEL_IMP
        GROUP_NPOW
        GROUP_POW
        GROUP_POW_0
        GROUP_POW_1
        GROUP_POW_2
        GROUP_POW_ADD
        GROUP_POW_ID
        GROUP_POW_MUL
        GROUP_POW_SUB
        GROUP_POW_SUBGROUP_GENERATED
        GROUP_POW_SUB_ALT
        GROUP_SETMUL_SYM
        GROUP_ZPOW
        GROUP_ZPOW_0
        GROUP_ZPOW_1
        GROUP_ZPOW_2
        GROUP_ZPOW_ADD
        GROUP_ZPOW_ID
        GROUP_ZPOW_MUL
        GROUP_ZPOW_NEG
        GROUP_ZPOW_SUB
        GROUP_ZPOW_SUBGROUP_GENERATED
        GROUP_ZPOW_SUB_ALT
        INFINITE_CYCLIC_SUBGROUP
        INFINITE_CYCLIC_SUBGROUP_ALT
        INTEGER_GROUP
        IN_SUBGROUP_DIV
        IN_SUBGROUP_ID
        IN_SUBGROUP_INV
        IN_SUBGROUP_MUL
        IN_SUBGROUP_POW
        IN_SUBGROUP_ZPOW
        ISOMORPHIC_GROUP_ABELIANNESS
        ISOMORPHIC_GROUP_CARD_EQ
        ISOMORPHIC_GROUP_CYCLICITY
        ISOMORPHIC_GROUP_INFINITE_CYCLIC_GROUPS
        ISOMORPHIC_GROUP_INFINITE_CYCLIC_INTEGER
        MONOIDAL_FRAG_ADD
        NEUTRAL_FRAG_ADD
        NO_PROPER_SUBGROUPS_IMP_CYCLIC
        QUOTIENT_GROUP_DIV
        QUOTIENT_GROUP_POW
        QUOTIENT_GROUP_ZPOW
        SUBGROUP_GENERATED_BY_SUBGROUP_GENERATED
        SUBGROUP_OF_CYCLIC_GROUP
        SUBGROUP_OF_CYCLIC_GROUP_EXPLICIT
        SUBGROUP_OF_POWERS
        SUBGROUP_SETMUL
        TRIVIAL_GROUP_SUBSET
        TRIVIAL_HOMOMORPHISM_GROUP_IMAGE
        TRIVIAL_HOMOMORPHISM_GROUP_KERNEL
        TRIVIAL_HOMOMORPHISM_TRIVIAL
        TRIVIAL_IMP_ABELIAN_GROUP
        TRIVIAL_IMP_CYCLIC_GROUP
        abelian_group
        cyclic_group
        frag_0
        frag_add
        frag_cmul
        frag_extend
        frag_neg
        frag_of
        frag_sub
        frag_support
        frag_tybij
        free_abelian_group
        group_pow
        group_zpow
        integer_group
        trivial_homomorphism

Library/grouptheory.ml
@@ -2,6 +2,12 @@
 (* Simple formulation of group theory with a type of "(A)group".             *)
 (* ========================================================================= *)
 
+needs "Library/frag.ml";;       (* Used eventually for free Abelian groups   *)
+
+(* ------------------------------------------------------------------------- *)
+(* Basic type of groups.                                                     *)
+(* ------------------------------------------------------------------------- *)
+
 let group_tybij =
   let eth = prove
    (`?s (z:A) n a.
@@ -27,32 +33,32 @@ let group_id = new_definition
 let group_inv = new_definition
  `(group_inv:(A)group->A->A) = \g. FST(SND(SND(group_operations g)))`;;
 
-let group_op = new_definition
- `(group_op:(A)group->A->A->A) = \g. SND(SND(SND(group_operations g)))`;;
+let group_mul = new_definition
+ `(group_mul:(A)group->A->A->A) = \g. SND(SND(SND(group_operations g)))`;;
 
-let ([GROUP_ID; GROUP_INV; GROUP_OP; GROUP_OP_ASSOC;
-      GROUP_OP_LID; GROUP_OP_RID; GROUP_OP_LINV; GROUP_OP_RINV] as
+let ([GROUP_ID; GROUP_INV; GROUP_MUL; GROUP_MUL_ASSOC;
+      GROUP_MUL_LID; GROUP_MUL_RID; GROUP_MUL_LINV; GROUP_MUL_RINV] as
      GROUP_PROPERTIES) = (CONJUNCTS o prove)
  (`(!G:A group. group_id G IN group_carrier G) /\
    (!G x:A. x IN group_carrier G ==> group_inv G x IN group_carrier G) /\
    (!G x y:A. x IN group_carrier G /\ y IN group_carrier G
-              ==> group_op G x y IN group_carrier G) /\
+              ==> group_mul G x y IN group_carrier G) /\
    (!G x y z:A. x IN group_carrier G /\
                 y IN group_carrier G /\
                 z IN group_carrier G
-                ==> group_op G x (group_op G y z) =
-                    group_op G (group_op G x y) z) /\
-   (!G x:A. x IN group_carrier G ==> group_op G (group_id G) x = x) /\
-   (!G x:A. x IN group_carrier G ==> group_op G x (group_id G) = x) /\
+                ==> group_mul G x (group_mul G y z) =
+                    group_mul G (group_mul G x y) z) /\
+   (!G x:A. x IN group_carrier G ==> group_mul G (group_id G) x = x) /\
+   (!G x:A. x IN group_carrier G ==> group_mul G x (group_id G) = x) /\
    (!G x:A. x IN group_carrier G
-            ==> group_op G (group_inv G x) x = group_id G) /\
+            ==> group_mul G (group_inv G x) x = group_id G) /\
    (!G x:A. x IN group_carrier G
-            ==> group_op G x(group_inv G x) = group_id G)`,
+            ==> group_mul G x(group_inv G x) = group_id G)`,
   REWRITE_TAC[AND_FORALL_THM] THEN GEN_TAC THEN
   MP_TAC(SPEC `G:A group` (MATCH_MP(MESON[]
    `(!a. mk(dest a) = a) /\ (!r. P r <=> dest(mk r) = r)
     ==> !a. P(dest a)`) group_tybij)) THEN
-  REWRITE_TAC[group_carrier; group_id; group_inv; group_op] THEN
+  REWRITE_TAC[group_carrier; group_id; group_inv; group_mul] THEN
   SIMP_TAC[]);;
 
 let GROUPS_EQ = prove
@@ -61,10 +67,10 @@ let GROUPS_EQ = prove
         group_carrier G = group_carrier H /\
         group_id G = group_id H /\
         group_inv G = group_inv H /\
-        group_op G = group_op H`,
+        group_mul G = group_mul H`,
   REWRITE_TAC[MESON[group_tybij]
    `g = h <=> group_operations g = group_operations h`] THEN
-  REWRITE_TAC[group_carrier;group_id;group_inv;group_op] THEN
+  REWRITE_TAC[group_carrier;group_id;group_inv;group_mul] THEN
   REWRITE_TAC[GSYM PAIR_EQ]);;
 
 let GROUP_CARRIER_NONEMPTY = prove
@@ -82,13 +88,13 @@ let SINGLETON_GROUP = prove
  (`(!a:A. group_carrier(singleton_group a) = {a}) /\
    (!a:A. group_id(singleton_group a) = a) /\
    (!a:A. group_inv(singleton_group a) = \x. a) /\
-   (!a:A. group_op(singleton_group a) = \x y. a)`,
+   (!a:A. group_mul(singleton_group a) = \x y. a)`,
   REWRITE_TAC[AND_FORALL_THM] THEN GEN_TAC THEN
   MP_TAC(fst(EQ_IMP_RULE
    (ISPEC(rand(rand(snd(strip_forall(concl singleton_group)))))
    (CONJUNCT2 group_tybij)))) THEN
   REWRITE_TAC[GSYM singleton_group] THEN SIMP_TAC[IN_SING] THEN
-  SIMP_TAC[group_carrier; group_id; group_inv; group_op]);;
+  SIMP_TAC[group_carrier; group_id; group_inv; group_mul]);;
 
 let trivial_group = new_definition
  `trivial_group G <=> group_carrier G = {group_id G}`;;
@@ -96,6 +102,10 @@ let trivial_group = new_definition
 let TRIVIAL_GROUP_SINGLETON_GROUP = prove
  (`!a:A. trivial_group(singleton_group a)`,
   REWRITE_TAC[trivial_group; SINGLETON_GROUP]);;
+
+let TRIVIAL_GROUP_SUBSET = prove
+ (`!G:A group. trivial_group G <=> group_carrier G SUBSET {group_id G}`,
+  SIMP_TAC[trivial_group; GSYM SUBSET_ANTISYM_EQ; SING_SUBSET; GROUP_ID]);;
 
 let TRIVIAL_GROUP = prove
  (`!G:A group. trivial_group G <=> ?a. group_carrier G = {a}`,
@@ -115,124 +125,139 @@ let TRIVIAL_GROUP_ALT = prove
 let opposite_group = new_definition
  `opposite_group(G:A group) =
         group(group_carrier G,group_id G,group_inv G,
-              \x y. group_op G y x)`;;
+              \x y. group_mul G y x)`;;
 
 let OPPOSITE_GROUP = prove
  (`!G:A group.
         group_carrier(opposite_group G) = group_carrier G /\
         group_id(opposite_group G) = group_id G /\
         group_inv(opposite_group G) = group_inv G /\
-        group_op(opposite_group G) = \x y. group_op G y x`,
+        group_mul(opposite_group G) = \x y. group_mul G y x`,
   GEN_TAC THEN
   MP_TAC(fst(EQ_IMP_RULE
    (ISPEC(rand(rand(snd(strip_forall(concl opposite_group)))))
    (CONJUNCT2 group_tybij)))) THEN
   REWRITE_TAC[GSYM opposite_group] THEN ANTS_TAC THENL
    [SIMP_TAC GROUP_PROPERTIES;
-    SIMP_TAC[group_carrier; group_id; group_inv; group_op]]);;
+    SIMP_TAC[group_carrier; group_id; group_inv; group_mul]]);;
 
 let OPPOSITE_OPPOSITE_GROUP = prove
  (`!G:A group. opposite_group (opposite_group G) = G`,
   GEN_TAC THEN ONCE_REWRITE_TAC[opposite_group] THEN
   REWRITE_TAC[OPPOSITE_GROUP; ETA_AX] THEN
   GEN_REWRITE_TAC RAND_CONV [GSYM(CONJUNCT1 group_tybij)] THEN
-  AP_TERM_TAC THEN REWRITE_TAC[group_carrier; group_id; group_inv; group_op]);;
+  AP_TERM_TAC THEN REWRITE_TAC[group_carrier; group_id; group_inv; group_mul]);;
 
 let OPPOSITE_GROUP_INV = prove
  (`!G x:A. group_inv(opposite_group G) x = group_inv G x`,
   REWRITE_TAC[OPPOSITE_GROUP]);;
 
-let OPPOSITE_GROUP_OP = prove
- (`!G x y:A. group_op(opposite_group G) x y = group_op G y x`,
+let OPPOSITE_GROUP_MUL = prove
+ (`!G x y:A. group_mul(opposite_group G) x y = group_mul G y x`,
   REWRITE_TAC[OPPOSITE_GROUP]);;
 
 (* ------------------------------------------------------------------------- *)
-(* Derived operations and derived properties.                                *)
+(* Derived operations and derived properties, including separate "powers"    *)
+(* for natural number (group_pow) and integer (group_zpow) indices.          *)
 (* ------------------------------------------------------------------------- *)
 
 let group_div = new_definition
- `group_div G x y = group_op G x (group_inv G y)`;;
+ `group_div G x y = group_mul G x (group_inv G y)`;;
 
 let GROUP_DIV = prove
  (`!G x y:A.
         x IN group_carrier G /\ y IN group_carrier G
         ==> (group_div G x y) IN group_carrier G`,
-  SIMP_TAC[group_div; GROUP_OP; GROUP_INV]);;
+  SIMP_TAC[group_div; GROUP_MUL; GROUP_INV]);;
 
-let GROUP_OP_LCANCEL = prove
+let GROUP_MUL_LCANCEL = prove
  (`!G x y z:A.
         x IN group_carrier G /\ y IN group_carrier G /\ z IN group_carrier G
-        ==> (group_op G x y = group_op G x z <=> y = z)`,
+        ==> (group_mul G x y = group_mul G x z <=> y = z)`,
   REPEAT STRIP_TAC THEN EQ_TAC THEN DISCH_TAC THEN ASM_REWRITE_TAC[] THEN
-  FIRST_X_ASSUM(MP_TAC o AP_TERM `group_op G (group_inv G x):A->A`) THEN
-  ASM_SIMP_TAC[GROUP_OP_ASSOC; GROUP_INV; GROUP_OP_LINV; GROUP_OP_LID]);;
+  FIRST_X_ASSUM(MP_TAC o AP_TERM `group_mul G (group_inv G x):A->A`) THEN
+  ASM_SIMP_TAC[GROUP_MUL_ASSOC; GROUP_INV; GROUP_MUL_LINV; GROUP_MUL_LID]);;
 
-let GROUP_OP_RCANCEL = prove
+let GROUP_MUL_LCANCEL_IMP = prove
+ (`!G x y z:A.
+        x IN group_carrier G /\ y IN group_carrier G /\ z IN group_carrier G /\
+        group_mul G x y = group_mul G x z
+        ==> y = z`,
+  MESON_TAC[GROUP_MUL_LCANCEL]);;
+
+let GROUP_MUL_RCANCEL = prove
  (`!G x y z:A.
         x IN group_carrier G /\ y IN group_carrier G /\ z IN group_carrier G
-        ==> (group_op G x z = group_op G y z <=> x = y)`,
-  ONCE_REWRITE_TAC[GSYM OPPOSITE_GROUP_OP] THEN
-  SIMP_TAC[GROUP_OP_LCANCEL; OPPOSITE_GROUP]);;
+        ==> (group_mul G x z = group_mul G y z <=> x = y)`,
+  ONCE_REWRITE_TAC[GSYM OPPOSITE_GROUP_MUL] THEN
+  SIMP_TAC[GROUP_MUL_LCANCEL; OPPOSITE_GROUP]);;
+
+let GROUP_MUL_RCANCEL_IMP = prove
+ (`!G x y z:A.
+        x IN group_carrier G /\ y IN group_carrier G /\ z IN group_carrier G /\
+        group_mul G x z = group_mul G y z
+        ==> x = y`,
+  MESON_TAC[GROUP_MUL_RCANCEL]);;
 
 let GROUP_LID_UNIQUE = prove
  (`!G x y:A.
-        x IN group_carrier G /\ y IN group_carrier G /\ group_op G x y = y
+        x IN group_carrier G /\ y IN group_carrier G /\ group_mul G x y = y
         ==> x = group_id G`,
-  MESON_TAC[GROUP_OP_RCANCEL; GROUP_OP_LID; GROUP_OP; GROUP_ID]);;
+  MESON_TAC[GROUP_MUL_RCANCEL; GROUP_MUL_LID; GROUP_MUL; GROUP_ID]);;
 
 let GROUP_RID_UNIQUE = prove
  (`!G x y:A.
-        x IN group_carrier G /\ y IN group_carrier G /\ group_op G x y = x
+        x IN group_carrier G /\ y IN group_carrier G /\ group_mul G x y = x
         ==> y = group_id G`,
-  MESON_TAC[GROUP_OP_LCANCEL; GROUP_OP_RID; GROUP_OP; GROUP_ID]);;
+  MESON_TAC[GROUP_MUL_LCANCEL; GROUP_MUL_RID; GROUP_MUL; GROUP_ID]);;
 
 let GROUP_LID_EQ = prove
  (`!G x y:A.
         x IN group_carrier G /\ y IN group_carrier G
-        ==> (group_op G x y = y <=> x = group_id G)`,
-  MESON_TAC[GROUP_LID_UNIQUE; GROUP_OP_LID]);;
+        ==> (group_mul G x y = y <=> x = group_id G)`,
+  MESON_TAC[GROUP_LID_UNIQUE; GROUP_MUL_LID]);;
 
 let GROUP_RID_EQ = prove
  (`!G x y:A.
         x IN group_carrier G /\ y IN group_carrier G
-        ==> (group_op G x y = x <=> y = group_id G)`,
-  MESON_TAC[GROUP_RID_UNIQUE; GROUP_OP_RID]);;
+        ==> (group_mul G x y = x <=> y = group_id G)`,
+  MESON_TAC[GROUP_RID_UNIQUE; GROUP_MUL_RID]);;
 
 let GROUP_LINV_UNIQUE = prove
  (`!G x y:A.
         x IN group_carrier G /\ y IN group_carrier G /\
-        group_op G x y = group_id G
+        group_mul G x y = group_id G
         ==> group_inv G x = y`,
-  MESON_TAC[GROUP_OP_LCANCEL; GROUP_INV; GROUP_OP_RINV]);;
+  MESON_TAC[GROUP_MUL_LCANCEL; GROUP_INV; GROUP_MUL_RINV]);;
 
 let GROUP_RINV_UNIQUE = prove
  (`!G x y:A.
         x IN group_carrier G /\ y IN group_carrier G /\
-        group_op G x y = group_id G
+        group_mul G x y = group_id G
         ==> group_inv G y = x`,
-  MESON_TAC[GROUP_OP_RCANCEL; GROUP_INV; GROUP_OP_LINV]);;
+  MESON_TAC[GROUP_MUL_RCANCEL; GROUP_INV; GROUP_MUL_LINV]);;
 
 let GROUP_LINV_EQ = prove
  (`!G x y:A.
         x IN group_carrier G /\ y IN group_carrier G
-        ==> (group_inv G x = y <=> group_op G x y = group_id G)`,
-  MESON_TAC[GROUP_LINV_UNIQUE; GROUP_OP_RINV]);;
+        ==> (group_inv G x = y <=> group_mul G x y = group_id G)`,
+  MESON_TAC[GROUP_LINV_UNIQUE; GROUP_MUL_RINV]);;
 
 let GROUP_RINV_EQ = prove
  (`!G x y:A.
         x IN group_carrier G /\ y IN group_carrier G
-        ==> (group_inv G x = y <=> group_op G y x = group_id G)`,
-  MESON_TAC[GROUP_RINV_UNIQUE; GROUP_OP_LINV]);;
+        ==> (group_inv G x = y <=> group_mul G y x = group_id G)`,
+  MESON_TAC[GROUP_RINV_UNIQUE; GROUP_MUL_LINV]);;
 
 let GROUP_INV_INV = prove
  (`!G x:A. x IN group_carrier G ==> group_inv G (group_inv G x) = x`,
   REPEAT STRIP_TAC THEN MATCH_MP_TAC GROUP_LINV_UNIQUE THEN
-  ASM_SIMP_TAC[GROUP_INV; GROUP_OP_LINV]);;
+  ASM_SIMP_TAC[GROUP_INV; GROUP_MUL_LINV]);;
 
 let GROUP_INV_ID = prove
  (`!G:A group. group_inv G (group_id G) = group_id G`,
   GEN_TAC THEN MATCH_MP_TAC GROUP_LINV_UNIQUE THEN
-  SIMP_TAC[GROUP_ID; GROUP_OP_LID]);;
+  SIMP_TAC[GROUP_ID; GROUP_MUL_LID]);;
 
 let GROUP_INV_EQ_ID = prove
  (`!G x:A.
@@ -240,22 +265,22 @@ let GROUP_INV_EQ_ID = prove
         ==> (group_inv G x = group_id G <=> x = group_id G)`,
   MESON_TAC[GROUP_INV_INV; GROUP_INV_ID]);;
 
-let GROUP_INV_OP = prove
+let GROUP_INV_MUL = prove
  (`!G x y:A.
         x IN group_carrier G /\ y IN group_carrier G
-        ==> group_inv G (group_op G x y) =
-            group_op G (group_inv G y) (group_inv G x)`,
+        ==> group_inv G (group_mul G x y) =
+            group_mul G (group_inv G y) (group_inv G x)`,
   REPEAT STRIP_TAC THEN MATCH_MP_TAC GROUP_LINV_UNIQUE THEN
-  ASM_SIMP_TAC[GROUP_OP; GROUP_INV; GROUP_OP_ASSOC] THEN
+  ASM_SIMP_TAC[GROUP_MUL; GROUP_INV; GROUP_MUL_ASSOC] THEN
   W(MP_TAC o PART_MATCH (rand o rand)
-    GROUP_OP_ASSOC o lhand o lhand o snd) THEN
-  ASM_SIMP_TAC[GROUP_OP_RINV; GROUP_INV] THEN
+    GROUP_MUL_ASSOC o lhand o lhand o snd) THEN
+  ASM_SIMP_TAC[GROUP_MUL_RINV; GROUP_INV] THEN
   DISCH_THEN(SUBST1_TAC o SYM) THEN
-  ASM_SIMP_TAC[GROUP_OP_RINV; GROUP_INV; GROUP_OP_RID]);;
+  ASM_SIMP_TAC[GROUP_MUL_RINV; GROUP_INV; GROUP_MUL_RID]);;
 
 let GROUP_DIV_REFL = prove
  (`!G x:A. x IN group_carrier G ==> group_div G x x = group_id G`,
-  SIMP_TAC[group_div; GROUP_OP_RINV]);;
+  SIMP_TAC[group_div; GROUP_MUL_RINV]);;
 
 let GROUP_DIV_EQ_ID = prove
  (`!G x y:A.
@@ -264,7 +289,193 @@ let GROUP_DIV_EQ_ID = prove
   REPEAT STRIP_TAC THEN
   SUBGOAL_THEN `group_id G:A = group_div G y y` SUBST1_TAC THENL
    [ASM_SIMP_TAC[GROUP_DIV_REFL];
-    ASM_SIMP_TAC[group_div; GROUP_OP_RCANCEL; GROUP_INV]]);;
+    ASM_SIMP_TAC[group_div; GROUP_MUL_RCANCEL; GROUP_INV]]);;
+
+let group_pow = new_recursive_definition num_RECURSION
+ `group_pow G x 0 = group_id G /\
+  group_pow G x (SUC n) = group_mul G x (group_pow G x n)`;;
+
+let GROUP_POW = prove
+ (`!G (x:A) n. x IN group_carrier G ==> group_pow G x n IN group_carrier G`,
+  REWRITE_TAC[RIGHT_FORALL_IMP_THM] THEN
+  REPEAT GEN_TAC THEN DISCH_TAC THEN
+  INDUCT_TAC THEN ASM_SIMP_TAC[group_pow; GROUP_ID; GROUP_MUL]);;
+
+let GROUP_POW_0 = prove
+ (`!G (x:A). group_pow G x 0 = group_id G`,
+  REWRITE_TAC[group_pow]);;
+
+let GROUP_POW_1 = prove
+ (`!G x:A. x IN group_carrier G ==> group_pow G x 1 = x`,
+  SIMP_TAC[num_CONV `1`; group_pow; GROUP_MUL_RID]);;
+
+let GROUP_POW_2 = prove
+ (`!G x:A. x IN group_carrier G ==> group_pow G x 2 = group_mul G x x`,
+  SIMP_TAC[num_CONV `2`; num_CONV `1`; group_pow; GROUP_MUL_RID]);;
+
+let GROUP_POW_ID = prove
+ (`!n. group_pow G (group_id G) n = group_id G`,
+  INDUCT_TAC THEN ASM_SIMP_TAC[group_pow; GROUP_ID; GROUP_MUL_LID]);;
+
+let GROUP_POW_ADD = prove
+ (`!G (x:A) m n.
+        x IN group_carrier G
+        ==> group_pow G x (m + n) =
+            group_mul G (group_pow G x m) (group_pow G x n)`,
+  REWRITE_TAC[RIGHT_FORALL_IMP_THM] THEN
+  REPEAT GEN_TAC THEN DISCH_TAC THEN
+  INDUCT_TAC THEN
+  ASM_SIMP_TAC[group_pow; ADD_CLAUSES; GROUP_POW; GROUP_MUL_LID] THEN
+  ASM_SIMP_TAC[GROUP_MUL_ASSOC; GROUP_POW]);;
+
+let GROUP_POW_SUB = prove
+ (`!G (x:A) m n.
+        x IN group_carrier G /\ n <= m
+        ==> group_pow G x (m - n) =
+            group_div G (group_pow G x m) (group_pow G x n)`,
+  REPEAT STRIP_TAC THEN MATCH_MP_TAC GROUP_MUL_RCANCEL_IMP THEN
+  MAP_EVERY EXISTS_TAC [`G:A group`; `group_pow G x n:A`] THEN
+  ASM_SIMP_TAC[GROUP_POW; GROUP_MUL; GROUP_INV; group_div;
+               GSYM GROUP_MUL_ASSOC; GROUP_MUL_LINV; GROUP_MUL_RID;
+               GSYM GROUP_POW_ADD; SUB_ADD]);;
+
+let GROUP_POW_SUB_ALT = prove
+ (`!G (x:A) m n.
+        x IN group_carrier G /\ n <= m
+        ==> group_pow G x (m - n) =
+            group_mul G (group_inv G (group_pow G x n)) (group_pow G x m)`,
+  REPEAT STRIP_TAC THEN MATCH_MP_TAC GROUP_MUL_LCANCEL_IMP THEN
+  MAP_EVERY EXISTS_TAC [`G:A group`; `group_pow G x n:A`] THEN
+  ASM_SIMP_TAC[GROUP_POW; GROUP_MUL; GROUP_INV; group_div; GROUP_MUL_ASSOC;
+               GROUP_MUL_RINV; GROUP_MUL_LID; GSYM GROUP_POW_ADD;
+               ARITH_RULE `n:num <= m ==> n + m - n = m`]);;
+
+let GROUP_INV_POW = prove
+ (`!G (x:A) n.
+        x IN group_carrier G
+        ==> group_inv G (group_pow G x n) = group_pow G (group_inv G x) n`,
+  REWRITE_TAC[RIGHT_FORALL_IMP_THM] THEN REPEAT GEN_TAC THEN DISCH_TAC THEN
+  INDUCT_TAC THEN REWRITE_TAC[CONJUNCT1 group_pow; GROUP_INV_ID] THEN
+  GEN_REWRITE_TAC (RAND_CONV o RAND_CONV) [ARITH_RULE `SUC n = 1 + n`] THEN
+  ASM_SIMP_TAC[ADD1; GROUP_POW_ADD; GROUP_INV; GROUP_INV_MUL; GROUP_POW;
+               GROUP_POW_1]);;
+
+let GROUP_POW_MUL = prove
+ (`!G (x:A) m n.
+        x IN group_carrier G
+        ==> group_pow G x (m * n) = group_pow G (group_pow G x m) n`,
+  REWRITE_TAC[RIGHT_FORALL_IMP_THM] THEN
+  REPEAT GEN_TAC THEN DISCH_TAC THEN GEN_TAC THEN
+  INDUCT_TAC THEN REWRITE_TAC[GROUP_POW_0; MULT_CLAUSES] THEN
+  ASM_SIMP_TAC[GROUP_POW_ADD; CONJUNCT2 group_pow]);;
+
+let group_zpow = new_definition
+ `group_zpow G (x:A) n =
+    if &0 <= n then group_pow G x (num_of_int n)
+    else group_inv G (group_pow G x (num_of_int(--n)))`;;
+
+let GROUP_ZPOW = prove
+ (`!G (x:A) n. x IN group_carrier G ==> group_zpow G x n IN group_carrier G`,
+  REPEAT STRIP_TAC THEN REWRITE_TAC[group_zpow] THEN
+  COND_CASES_TAC THEN ASM_SIMP_TAC[GROUP_POW; GROUP_INV]);;
+
+let GROUP_NPOW = prove
+ (`!G (x:A) n. group_zpow G x (&n) = group_pow G x n`,
+  REWRITE_TAC[NUM_OF_INT_OF_NUM; group_zpow; INT_POS]);;
+
+let GROUP_ZPOW_0 = prove
+ (`!G (x:A). group_zpow G x (&0) = group_id G`,
+  REWRITE_TAC[GROUP_NPOW; GROUP_POW_0]);;
+
+let GROUP_ZPOW_1 = prove
+ (`!G x:A. x IN group_carrier G ==> group_zpow G x (&1) = x`,
+  REWRITE_TAC[GROUP_NPOW; GROUP_POW_1]);;
+
+let GROUP_ZPOW_2 = prove
+ (`!G x:A. x IN group_carrier G ==> group_zpow G x (&2) = group_mul G x x`,
+  REWRITE_TAC[GROUP_NPOW; GROUP_POW_2]);;
+
+let GROUP_ZPOW_ID = prove
+ (`!n. group_zpow G (group_id G) n = group_id G`,
+  GEN_TAC THEN REWRITE_TAC[group_zpow; GROUP_POW_ID; GROUP_INV_ID; COND_ID]);;
+
+let GROUP_ZPOW_NEG = prove
+ (`!G (x:A) n.
+        x IN group_carrier G
+        ==> group_zpow G x (--n) = group_inv G (group_zpow G x n)`,
+  REPEAT STRIP_TAC THEN ASM_CASES_TAC `n:int = &0` THEN
+  ASM_REWRITE_TAC[INT_NEG_0; GROUP_NPOW; group_pow; GROUP_INV_ID] THEN
+  REWRITE_TAC[group_zpow; INT_NEG_NEG] THEN
+  ASM_SIMP_TAC[INT_ARITH `~(n:int = &0) ==> (&0 <= --n <=> ~(&0 <= n))`] THEN
+  ASM_CASES_TAC `&0:int <= n` THEN
+  ASM_SIMP_TAC[GROUP_INV_INV; GROUP_POW]);;
+
+let GROUP_ZPOW_ADD = prove
+ (`!G (x:A) m n.
+        x IN group_carrier G
+        ==> group_zpow G x (m + n) =
+            group_mul G (group_zpow G x m) (group_zpow G x n)`,
+  REPEAT STRIP_TAC THEN
+  DISJ_CASES_THEN MP_TAC(SPEC `n:int` INT_IMAGE) THEN
+  DISJ_CASES_THEN MP_TAC(SPEC `m:int` INT_IMAGE) THEN
+  REWRITE_TAC[LEFT_IMP_EXISTS_THM] THEN
+  X_GEN_TAC `p:num` THEN DISCH_THEN SUBST1_TAC THEN
+  X_GEN_TAC `q:num` THEN DISCH_THEN SUBST1_TAC THEN
+  ASM_SIMP_TAC[GSYM INT_NEG_ADD; GROUP_ZPOW_NEG; GROUP_NPOW;
+               INT_OF_NUM_ADD] THEN
+  REPEAT CONJ_TAC THENL
+   [ASM_SIMP_TAC[GROUP_POW_ADD];
+    DISJ_CASES_TAC(ARITH_RULE `p:num <= q \/ q <= p`) THENL
+     [ASM_REWRITE_TAC[INT_ARITH `--x + y:int = y - x`];
+      ASM_REWRITE_TAC[INT_ARITH `--x + y:int = --(x - y)`]] THEN
+    ASM_SIMP_TAC[GROUP_ZPOW_NEG; INT_OF_NUM_SUB; GROUP_NPOW] THEN
+    ASM_SIMP_TAC[GROUP_POW_SUB_ALT; GROUP_INV_MUL; GROUP_INV_INV;
+                 GROUP_POW; GROUP_INV; GROUP_MUL];
+    DISJ_CASES_TAC(ARITH_RULE `q:num <= p \/ p <= q`) THENL
+     [ASM_REWRITE_TAC[INT_ARITH `y + --x:int = y - x`];
+      ASM_REWRITE_TAC[INT_ARITH `y + --x:int = --(x - y)`]] THEN
+    ASM_SIMP_TAC[GROUP_ZPOW_NEG; INT_OF_NUM_SUB; GROUP_NPOW] THEN
+    ASM_SIMP_TAC[GROUP_POW_SUB; GROUP_INV_MUL; GROUP_INV_INV;
+                 GROUP_POW; GROUP_INV; GROUP_MUL; group_div];
+    ONCE_REWRITE_TAC[ADD_SYM] THEN
+    ASM_SIMP_TAC[GROUP_POW_ADD; GROUP_INV_MUL; GROUP_POW]]);;
+
+let GROUP_ZPOW_SUB = prove
+ (`!G (x:A) m n.
+        x IN group_carrier G
+        ==> group_zpow G x (m - n) =
+            group_div G (group_zpow G x m) (group_zpow G x n)`,
+  SIMP_TAC[group_div; INT_SUB; GROUP_ZPOW_ADD; GROUP_ZPOW_NEG]);;
+
+let GROUP_ZPOW_SUB_ALT = prove
+ (`!G (x:A) m n.
+        x IN group_carrier G
+        ==> group_zpow G x (m - n) =
+            group_mul G (group_inv G (group_zpow G x n)) (group_zpow G x m)`,
+  REWRITE_TAC[INT_ARITH `x - y:int = --y + x`] THEN
+  SIMP_TAC[GROUP_ZPOW_ADD; GROUP_ZPOW_NEG]);;
+
+let GROUP_INV_ZPOW = prove
+ (`!G (x:A) n.
+        x IN group_carrier G
+        ==> group_inv G (group_zpow G x n) = group_zpow G (group_inv G x) n`,
+  REPEAT STRIP_TAC THEN REWRITE_TAC[group_zpow] THEN
+  COND_CASES_TAC THEN ASM_SIMP_TAC[GROUP_INV_POW]);;
+
+let GROUP_ZPOW_MUL = prove
+ (`!G (x:A) m n.
+        x IN group_carrier G
+        ==> group_zpow G x (m * n) = group_zpow G (group_zpow G x m) n`,
+  REPEAT STRIP_TAC THEN
+  DISJ_CASES_THEN MP_TAC(SPEC `n:int` INT_IMAGE) THEN
+  DISJ_CASES_THEN MP_TAC(SPEC `m:int` INT_IMAGE) THEN
+  REWRITE_TAC[LEFT_IMP_EXISTS_THM] THEN
+  X_GEN_TAC `p:num` THEN DISCH_THEN SUBST1_TAC THEN
+  X_GEN_TAC `q:num` THEN DISCH_THEN SUBST1_TAC THEN
+  ASM_REWRITE_TAC[INT_MUL_LNEG; INT_MUL_RNEG; INT_NEG_NEG] THEN
+  ASM_SIMP_TAC[GROUP_ZPOW_NEG; INT_OF_NUM_MUL; GROUP_NPOW;
+               GROUP_INV; GROUP_POW; GROUP_POW_MUL; GROUP_INV_POW;
+               GROUP_INV_INV]);;
 
 (* ------------------------------------------------------------------------- *)
 (* Subgroups. We treat them as *sets* which seems to be a common convention. *)
@@ -279,7 +490,34 @@ let subgroup_of = new_definition
         s SUBSET group_carrier G /\
         group_id G IN s /\
         (!x. x IN s ==> group_inv G x IN s) /\
-        (!x y. x IN s /\ y IN s ==> group_op G x y IN s)`;;
+        (!x y. x IN s /\ y IN s ==> group_mul G x y IN s)`;;
+
+let IN_SUBGROUP_ID = prove
+ (`!G h:A->bool. h subgroup_of G ==> group_id G IN h`,
+  SIMP_TAC[subgroup_of]);;
+
+let IN_SUBGROUP_INV = prove
+ (`!G h x:A. h subgroup_of G /\ x IN h ==> group_inv G x IN h`,
+  SIMP_TAC[subgroup_of]);;
+
+let IN_SUBGROUP_MUL = prove
+ (`!G h x y:A. h subgroup_of G /\ x IN h /\ y IN h ==> group_mul G x y IN h`,
+  SIMP_TAC[subgroup_of]);;
+
+let IN_SUBGROUP_DIV = prove
+ (`!G h x y:A. h subgroup_of G /\ x IN h /\ y IN h ==> group_div G x y IN h`,
+  SIMP_TAC[group_div; IN_SUBGROUP_MUL; IN_SUBGROUP_INV]);;
+
+let IN_SUBGROUP_POW = prove
+ (`!G h (x:A) n. h subgroup_of G /\ x IN h ==> group_pow G x n IN h`,
+  REWRITE_TAC[RIGHT_FORALL_IMP_THM] THEN
+  REPEAT GEN_TAC THEN DISCH_TAC THEN INDUCT_TAC THEN
+  ASM_SIMP_TAC[group_pow; IN_SUBGROUP_ID; IN_SUBGROUP_MUL]);;
+
+let IN_SUBGROUP_ZPOW = prove
+ (`!G h (x:A) n. h subgroup_of G /\ x IN h ==> group_zpow G x n IN h`,
+  REPEAT STRIP_TAC THEN REWRITE_TAC[group_zpow] THEN
+  COND_CASES_TAC THEN ASM_SIMP_TAC[IN_SUBGROUP_INV; IN_SUBGROUP_POW]);;
 
 let SUBGROUP_OF_INTERS = prove
  (`!G (gs:(A->bool)->bool).
@@ -316,7 +554,7 @@ let CARRIER_SUBGROUP_OF = prove
 let subgroup_generated = new_definition
  `subgroup_generated G (s:A->bool) =
       group(INTERS {h | h subgroup_of G /\ (group_carrier G INTER s) SUBSET h},
-            group_id G,group_inv G,group_op G)`;;
+            group_id G,group_inv G,group_mul G)`;;
 
 let SUBGROUP_GENERATED = prove
  (`(!G s:A->bool.
@@ -324,7 +562,7 @@ let SUBGROUP_GENERATED = prove
           INTERS {h | h subgroup_of G /\ (group_carrier G INTER s) SUBSET h}) /\
     (!G s:A->bool. group_id (subgroup_generated G s) = group_id G) /\
     (!G s:A->bool. group_inv (subgroup_generated G s) = group_inv G) /\
-    (!G s:A->bool. group_op (subgroup_generated G s) = group_op G)`,
+    (!G s:A->bool. group_mul (subgroup_generated G s) = group_mul G)`,
   REWRITE_TAC[AND_FORALL_THM] THEN REPEAT GEN_TAC THEN
   MP_TAC(fst(EQ_IMP_RULE
    (ISPEC(rand(rand(snd(strip_forall(concl subgroup_generated)))))
@@ -338,7 +576,21 @@ let SUBGROUP_GENERATED = prove
     REWRITE_TAC[INTER_SUBSET; SUBSET_REFL; CARRIER_SUBGROUP_OF] THEN
     MESON_TAC GROUP_PROPERTIES;
     DISCH_TAC THEN
-    ASM_REWRITE_TAC[group_carrier; group_id; group_inv; group_op]]);;
+    ASM_REWRITE_TAC[group_carrier; group_id; group_inv; group_mul]]);;
+
+let GROUP_DIV_SUBGROUP_GENERATED = prove
+ (`!G s:A->bool. group_div (subgroup_generated G s) = group_div G`,
+  REWRITE_TAC[FUN_EQ_THM; group_div; SUBGROUP_GENERATED]);;
+
+let GROUP_POW_SUBGROUP_GENERATED = prove
+ (`!G s:A->bool. group_pow (subgroup_generated G s) = group_pow G`,
+  REPEAT GEN_TAC THEN REWRITE_TAC[FUN_EQ_THM] THEN GEN_TAC THEN
+  INDUCT_TAC THEN ASM_REWRITE_TAC[group_pow; SUBGROUP_GENERATED]);;
+
+let GROUP_ZPOW_SUBGROUP_GENERATED = prove
+ (`!G s:A->bool. group_zpow (subgroup_generated G s) = group_zpow G`,
+  REWRITE_TAC[group_zpow; GROUP_POW_SUBGROUP_GENERATED;
+              SUBGROUP_GENERATED; FUN_EQ_THM]);;
 
 let SUBGROUP_GENERATED_RESTRICT = prove
  (`!G s:A->bool.
@@ -372,7 +624,7 @@ let SUBGROUP_GENERATED_INDUCT = prove
         (!x. x IN group_carrier G /\ x IN s ==> P x) /\
         P(group_id G) /\
         (!x. P x ==> P(group_inv G x)) /\
-        (!x y. P x /\ P y ==> P(group_op G x y))
+        (!x y. P x /\ P y ==> P(group_mul G x y))
         ==> !x. x IN group_carrier(subgroup_generated G s) ==> P x`,
   REPEAT GEN_TAC THEN REWRITE_TAC[GSYM IN_INTER] THEN
   ONCE_REWRITE_TAC[SUBGROUP_GENERATED_RESTRICT] THEN MP_TAC(SET_RULE
@@ -383,7 +635,7 @@ let SUBGROUP_GENERATED_INDUCT = prove
                  `s:A->bool`] SUBGROUP_GENERATED_MINIMAL) THEN
   ANTS_TAC THENL [ALL_TAC; SET_TAC[]] THEN
   CONJ_TAC THENL [ASM SET_TAC[]; ALL_TAC] THEN
-  ASM_SIMP_TAC[subgroup_of; IN_ELIM_THM; SUBSET; GROUP_OP; GROUP_INV;
+  ASM_SIMP_TAC[subgroup_of; IN_ELIM_THM; SUBSET; GROUP_MUL; GROUP_INV;
                GROUP_ID]);;
 
 let GROUP_CARRIER_SUBGROUP_GENERATED_SUBSET = prove
@@ -457,6 +709,18 @@ let TRIVIAL_GROUP_SUBGROUP_GENERATED_TRIVIAL = prove
   EXISTS_TAC `{group_id G:A}` THEN
   REWRITE_TAC[IN_ELIM_THM; TRIVIAL_SUBGROUP_OF] THEN ASM SET_TAC[]);;
 
+let SUBGROUP_GENERATED_BY_SUBGROUP_GENERATED = prove
+ (`!G s:A->bool.
+        subgroup_generated G (group_carrier(subgroup_generated G s)) =
+        subgroup_generated G s`,
+  REPEAT GEN_TAC THEN
+  REWRITE_TAC[GROUPS_EQ; CONJUNCT2 SUBGROUP_GENERATED] THEN
+  MATCH_MP_TAC SUBSET_ANTISYM THEN CONJ_TAC THENL
+   [MATCH_MP_TAC SUBGROUP_GENERATED_MINIMAL THEN
+    REWRITE_TAC[SUBGROUP_SUBGROUP_GENERATED; SUBSET_REFL];
+    MATCH_MP_TAC SUBGROUP_GENERATED_SUBSET_CARRIER_SUBSET THEN
+    REWRITE_TAC[GROUP_CARRIER_SUBGROUP_GENERATED_SUBSET]]);;
+
 (* ------------------------------------------------------------------------- *)
 (* Direct products and sums.                                                 *)
 (* ------------------------------------------------------------------------- *)
@@ -466,7 +730,7 @@ let prod_group = new_definition
         group((group_carrier G) CROSS (group_carrier G'),
               (group_id G,group_id G'),
               (\(x,x'). group_inv G x,group_inv G' x'),
-              (\(x,x') (y,y'). group_op G x y,group_op G' x' y'))`;;
+              (\(x,x') (y,y'). group_mul G x y,group_mul G' x' y'))`;;
 
 let PROD_GROUP = prove
  (`(!(G:A group) (G':B group).
@@ -478,8 +742,8 @@ let PROD_GROUP = prove
         group_inv (prod_group G G') =
           \(x,x'). group_inv G x,group_inv G' x') /\
    (!(G:A group) (G':B group).
-        group_op (prod_group G G') =
-          \(x,x') (y,y'). group_op G x y,group_op G' x' y')`,
+        group_mul (prod_group G G') =
+          \(x,x') (y,y'). group_mul G x y,group_mul G' x' y')`,
   REWRITE_TAC[AND_FORALL_THM] THEN REPEAT GEN_TAC THEN
   MP_TAC(fst(EQ_IMP_RULE
    (ISPEC(rand(rand(snd(strip_forall(concl prod_group)))))
@@ -488,14 +752,14 @@ let PROD_GROUP = prove
    [REWRITE_TAC[FORALL_PAIR_THM; IN_CROSS; PAIR_EQ] THEN
     SIMP_TAC GROUP_PROPERTIES;
     DISCH_TAC THEN
-    ASM_REWRITE_TAC[group_carrier; group_id; group_inv; group_op]]);;
+    ASM_REWRITE_TAC[group_carrier; group_id; group_inv; group_mul]]);;
 
 let product_group = new_definition
  `product_group k (G:K->A group) =
         group(cartesian_product k (\i. group_carrier(G i)),
               RESTRICTION k (\i. group_id (G i)),
               (\x. RESTRICTION k (\i. group_inv (G i) (x i))),
-              (\x y. RESTRICTION k (\i. group_op (G i) (x i) (y i))))`;;
+              (\x y. RESTRICTION k (\i. group_mul (G i) (x i) (y i))))`;;
 
 let PRODUCT_GROUP = prove
  (`(!k (G:K->A group).
@@ -508,8 +772,8 @@ let PRODUCT_GROUP = prove
         group_inv (product_group k G) =
           \x. RESTRICTION k (\i. group_inv (G i) (x i))) /\
    (!k (G:K->A group).
-        group_op (product_group k G) =
-          (\x y. RESTRICTION k (\i. group_op (G i) (x i) (y i))))`,
+        group_mul (product_group k G) =
+          (\x y. RESTRICTION k (\i. group_mul (G i) (x i) (y i))))`,
   REWRITE_TAC[AND_FORALL_THM] THEN REPEAT GEN_TAC THEN
   MP_TAC(fst(EQ_IMP_RULE
    (ISPEC(rand(rand(snd(strip_forall(concl product_group)))))
@@ -521,7 +785,7 @@ let PRODUCT_GROUP = prove
     REPEAT(COND_CASES_TAC THEN ASM_REWRITE_TAC[]) THEN
     ASM_SIMP_TAC GROUP_PROPERTIES;
     DISCH_TAC THEN
-    ASM_REWRITE_TAC[group_carrier; group_id; group_inv; group_op]]);;
+    ASM_REWRITE_TAC[group_carrier; group_id; group_inv; group_mul]]);;
 
 let SUBGROUP_SUM_GROUP = prove
  (`!k (G:K->A group).
@@ -531,7 +795,7 @@ let SUBGROUP_SUM_GROUP = prove
   REWRITE_TAC[subgroup_of; PRODUCT_GROUP; SUBSET_RESTRICT] THEN
   REWRITE_TAC[RESTRICTION; cartesian_product; IN_ELIM_THM; EXTENSIONAL] THEN
   ONCE_REWRITE_TAC[TAUT `p /\ ~q <=> ~(p ==> q)`] THEN
-  SIMP_TAC[GROUP_ID; GROUP_INV_EQ_ID; GROUP_INV; GROUP_OP] THEN
+  SIMP_TAC[GROUP_ID; GROUP_INV_EQ_ID; GROUP_INV; GROUP_MUL] THEN
   REWRITE_TAC[EMPTY_GSPEC; FINITE_EMPTY] THEN REPEAT GEN_TAC THEN
   DISCH_THEN(CONJUNCTS_THEN(CONJUNCTS_THEN2 STRIP_ASSUME_TAC MP_TAC)) THEN
   REWRITE_TAC[IMP_IMP; GSYM FINITE_UNION] THEN
@@ -540,7 +804,7 @@ let SUBGROUP_SUM_GROUP = prove
   GEN_TAC THEN GEN_REWRITE_TAC I [GSYM CONTRAPOS_THM] THEN
   REWRITE_TAC[DE_MORGAN_THM] THEN STRIP_TAC THEN
   REWRITE_TAC[TAUT `~p \/ q <=> p ==> q`] THEN
-  ASM_SIMP_TAC[GROUP_OP_LID; GROUP_ID]);;
+  ASM_SIMP_TAC[GROUP_MUL_LID; GROUP_ID]);;
 
 let sum_group = new_definition
   `sum_group k (G:K->A group) =
@@ -561,8 +825,8 @@ let SUM_GROUP = prove
         group_inv (sum_group k G) =
           \x. RESTRICTION k (\i. group_inv (G i) (x i))) /\
    (!k (G:K->A group).
-        group_op (sum_group k G) =
-          (\x y. RESTRICTION k (\i. group_op (G i) (x i) (y i))))`,
+        group_mul (sum_group k G) =
+          (\x y. RESTRICTION k (\i. group_mul (G i) (x i) (y i))))`,
   SIMP_TAC[sum_group; SUBGROUP_SUM_GROUP;
            CARRIER_SUBGROUP_GENERATED_SUBGROUP] THEN
   REWRITE_TAC[SUBGROUP_GENERATED; PRODUCT_GROUP]);;
@@ -578,7 +842,7 @@ let group_homomorphism = new_definition
         (!x. x IN group_carrier G
              ==> f(group_inv G x) = group_inv G' (f x)) /\
         (!x y. x IN group_carrier G /\ y IN group_carrier G
-               ==> f(group_op G x y) = group_op G' (f x) (f y))`;;
+               ==> f(group_mul G x y) = group_mul G' (f x) (f y))`;;
 
 let group_monomorphism = new_definition
  `group_monomorphism (G,G') (f:A->B) <=>
@@ -613,7 +877,7 @@ let GROUP_HOMOMORPHISM_EQ = prove
         (!x. x IN group_carrier G ==> f' x = f x)
         ==> group_homomorphism (G,H) f'`,
   REWRITE_TAC[group_homomorphism; SUBSET; FORALL_IN_IMAGE] THEN
-  SIMP_TAC[GROUP_ID; GROUP_INV; GROUP_OP]);;
+  SIMP_TAC[GROUP_ID; GROUP_INV; GROUP_MUL]);;
 
 let GROUP_MONOMORPHISM_EQ = prove
  (`!G H (f:A->B) f'.
@@ -621,7 +885,7 @@ let GROUP_MONOMORPHISM_EQ = prove
         (!x. x IN group_carrier G ==> f' x = f x)
         ==> group_monomorphism (G,H) f'`,
   REWRITE_TAC[group_monomorphism; group_homomorphism; SUBSET] THEN
-  SIMP_TAC[FORALL_IN_IMAGE; GROUP_ID; GROUP_INV; GROUP_OP] THEN
+  SIMP_TAC[FORALL_IN_IMAGE; GROUP_ID; GROUP_INV; GROUP_MUL] THEN
   MESON_TAC[]);;
 
 let GROUP_EPIMORPHISM_EQ = prove
@@ -630,7 +894,7 @@ let GROUP_EPIMORPHISM_EQ = prove
         (!x. x IN group_carrier G ==> f' x = f x)
         ==> group_epimorphism (G,H) f'`,
   REWRITE_TAC[group_epimorphism; group_homomorphism; SUBSET] THEN
-  SIMP_TAC[FORALL_IN_IMAGE; GROUP_ID; GROUP_INV; GROUP_OP] THEN
+  SIMP_TAC[FORALL_IN_IMAGE; GROUP_ID; GROUP_INV; GROUP_MUL] THEN
   SET_TAC[]);;
 
 let GROUP_ENDOMORPHISM_EQ = prove
@@ -647,7 +911,7 @@ let GROUP_ISOMORPHISMS_EQ = prove
         (!y. y IN group_carrier H ==> g' y = g y)
         ==> group_isomorphisms(G,H) (f',g')`,
   SIMP_TAC[group_isomorphisms; group_homomorphism; SUBSET] THEN
-  SIMP_TAC[FORALL_IN_IMAGE; GROUP_ID; GROUP_INV; GROUP_OP] THEN
+  SIMP_TAC[FORALL_IN_IMAGE; GROUP_ID; GROUP_INV; GROUP_MUL] THEN
   SET_TAC[]);;
 
 let GROUP_ISOMORPHISM_EQ = prove
@@ -676,19 +940,33 @@ let GROUP_HOMOMORPHISM = prove
         group_homomorphism (G,G') (f:A->B) <=>
         IMAGE f (group_carrier G) SUBSET group_carrier G' /\
         (!x y. x IN group_carrier G /\ y IN group_carrier G
-               ==> f(group_op G x y) = group_op G' (f x) (f y))`,
+               ==> f(group_mul G x y) = group_mul G' (f x) (f y))`,
   REPEAT GEN_TAC THEN REWRITE_TAC[group_homomorphism] THEN
   EQ_TAC THEN STRIP_TAC THEN ASM_REWRITE_TAC[] THEN
   RULE_ASSUM_TAC(REWRITE_RULE[SUBSET; FORALL_IN_IMAGE]) THEN
   MATCH_MP_TAC(TAUT `p /\ (p ==> q) ==> p /\ q`) THEN CONJ_TAC THENL
    [FIRST_X_ASSUM(MP_TAC o SPECL [`group_id G:A`; `group_id G:A`]) THEN
-    SIMP_TAC[GROUP_ID; GROUP_OP_LID] THEN
+    SIMP_TAC[GROUP_ID; GROUP_MUL_LID] THEN
     GEN_REWRITE_TAC LAND_CONV [EQ_SYM_EQ] THEN
     ASM_MESON_TAC[GROUP_LID_UNIQUE; GROUP_ID];
     REPEAT STRIP_TAC THEN CONV_TAC SYM_CONV THEN
     MATCH_MP_TAC GROUP_LINV_UNIQUE THEN
     FIRST_X_ASSUM(MP_TAC o SPECL [`x:A`; `group_inv G x:A`]) THEN
-    ASM_SIMP_TAC[GROUP_INV; GROUP_OP_RINV]]);;
+    ASM_SIMP_TAC[GROUP_INV; GROUP_MUL_RINV]]);;
+
+let GROUP_HOMOMORPHISM_INV = prove
+ (`!G G' (f:A->B).
+        group_homomorphism(G,G') f
+        ==> !x. x IN group_carrier G
+                ==> f(group_inv G x) = group_inv G' (f x)`,
+  SIMP_TAC[group_homomorphism]);;
+
+let GROUP_HOMOMORPHISM_MUL = prove
+ (`!G G' (f:A->B).
+        group_homomorphism(G,G') f
+        ==> !x y. x IN group_carrier G /\ y IN group_carrier G
+                  ==> f(group_mul G x y) = group_mul G' (f x) (f y)`,
+  SIMP_TAC[group_homomorphism]);;
 
 let GROUP_HOMOMORPHISM_DIV = prove
  (`!G G' (f:A->B).
@@ -696,7 +974,25 @@ let GROUP_HOMOMORPHISM_DIV = prove
         ==> !x y. x IN group_carrier G /\ y IN group_carrier G
                   ==> f(group_div G x y) = group_div G' (f x) (f y)`,
   REWRITE_TAC[group_homomorphism; group_div] THEN
-  MESON_TAC[GROUP_OP; GROUP_INV]);;
+  MESON_TAC[GROUP_MUL; GROUP_INV]);;
+
+let GROUP_HOMOMORPHISM_POW = prove
+ (`!G G' (f:A->B).
+        group_homomorphism(G,G') f
+        ==> !x n. x IN group_carrier G
+                  ==> f(group_pow G x n) = group_pow G' (f x) n`,
+  REPEAT GEN_TAC THEN REWRITE_TAC[group_homomorphism] THEN DISCH_TAC THEN
+  REWRITE_TAC[RIGHT_FORALL_IMP_THM] THEN GEN_TAC THEN DISCH_TAC THEN
+  INDUCT_TAC THEN ASM_SIMP_TAC[group_pow; GROUP_POW]);;
+
+let GROUP_HOMOMORPHISM_ZPOW = prove
+ (`!G G' (f:A->B).
+        group_homomorphism(G,G') f
+        ==> !x n. x IN group_carrier G
+                  ==> f(group_zpow G x n) = group_zpow G' (f x) n`,
+  REPEAT STRIP_TAC THEN REWRITE_TAC[group_zpow] THEN
+  COND_CASES_TAC THEN
+  ASM_MESON_TAC[GROUP_HOMOMORPHISM_POW; GROUP_HOMOMORPHISM_INV; GROUP_POW]);;
 
 let GROUP_HOMOMORPHISM_ID = prove
  (`!G:A group. group_homomorphism (G,G) (\x. x)`,
@@ -907,14 +1203,14 @@ let GROUP_ISOMORPHISM_INVERSE = prove
   SUBGOAL_THEN
    `!y. y IN group_carrier H ==> (f:A->B)(g y) = y`
   ASSUME_TAC THENL [ASM_MESON_TAC[]; ALL_TAC] THEN
-  ASM_MESON_TAC[GROUP_ID; GROUP_INV; GROUP_OP]);;
+  ASM_MESON_TAC[GROUP_ID; GROUP_INV; GROUP_MUL]);;
 
 let GROUP_ISOMORPHISMS_OPPOSITE_GROUP = prove
  (`!G:A group.
         group_isomorphisms(G,opposite_group G) (group_inv G,group_inv G)`,
   REWRITE_TAC[group_isomorphisms; group_homomorphism; OPPOSITE_GROUP] THEN
   REWRITE_TAC[SUBSET; FORALL_IN_IMAGE; GROUP_INV_ID] THEN
-  SIMP_TAC[GROUP_INV; GROUP_INV_OP; GROUP_INV_INV]);;
+  SIMP_TAC[GROUP_INV; GROUP_INV_MUL; GROUP_INV_INV]);;
 
 let GROUP_HOMOMORPHISM_FROM_TRIVIAL_GROUP = prove
  (`!(f:A->B) G H.
@@ -923,7 +1219,7 @@ let GROUP_HOMOMORPHISM_FROM_TRIVIAL_GROUP = prove
   REPEAT GEN_TAC THEN SIMP_TAC[trivial_group; group_homomorphism] THEN
   ASM_CASES_TAC `(f:A->B)(group_id G) = group_id H` THEN
   ASM_REWRITE_TAC[] THEN DISCH_THEN(K ALL_TAC) THEN
-  ASM_SIMP_TAC[IN_SING; GROUP_OP_LID; GROUP_ID; SUBSET; FORALL_IN_IMAGE;
+  ASM_SIMP_TAC[IN_SING; GROUP_MUL_LID; GROUP_ID; SUBSET; FORALL_IN_IMAGE;
                GROUP_INV_ID]);;
 
 let GROUP_MONOMORPHISM_FROM_TRIVIAL_GROUP = prove
@@ -1077,7 +1373,7 @@ let ISOMORPHIC_TO_TRIVIAL_GROUP = prove
     EXISTS_TAC `(\x. b):A->B` THEN
     ASM_REWRITE_TAC[group_homomorphism] THEN
     SIMP_TAC[IN_SING; IMAGE_CLAUSES; SUBSET_REFL] THEN
-    ASM_MESON_TAC[GROUP_ID; GROUP_INV; GROUP_OP; IN_SING]) in
+    ASM_MESON_TAC[GROUP_ID; GROUP_INV; GROUP_MUL; IN_SING]) in
   REWRITE_TAC[lemma] THEN ONCE_REWRITE_TAC[ISOMORPHIC_GROUP_SYM] THEN
   REWRITE_TAC[lemma]);;
 
@@ -1096,6 +1392,13 @@ let ISOMORPHIC_GROUP_PROD_GROUPS = prove
   REWRITE_TAC[LEFT_AND_EXISTS_THM; LEFT_IMP_EXISTS_THM] THEN
   REWRITE_TAC[GSYM GROUP_ISOMORPHISMS_PAIRED2] THEN MESON_TAC[]);;
 
+let ISOMORPHIC_GROUP_CARD_EQ = prove
+ (`!(G:A group) (H:B group).
+        G isomorphic_group H ==> group_carrier G =_c group_carrier H`,
+  REWRITE_TAC[isomorphic_group; GSYM GROUP_MONOMORPHISM_EPIMORPHISM] THEN
+  REWRITE_TAC[eq_c; group_monomorphism; group_epimorphism] THEN
+  REPEAT GEN_TAC THEN MATCH_MP_TAC MONO_EXISTS THEN SET_TAC[]);;
+
 (* ------------------------------------------------------------------------- *)
 (* Perform group operations setwise.                                         *)
 (* ------------------------------------------------------------------------- *)
@@ -1103,8 +1406,8 @@ let ISOMORPHIC_GROUP_PROD_GROUPS = prove
 let group_setinv = new_definition
  `group_setinv G g = {group_inv G x | x IN g}`;;
 
-let group_setop = new_definition
- `group_setop G g h = {group_op G x y | x IN g /\ y IN h}`;;
+let group_setmul = new_definition
+ `group_setmul G g h = {group_mul G x y | x IN g /\ y IN h}`;;
 
 let SUBGROUP_OF_SETWISE = prove
  (`!G s:A->bool.
@@ -1112,67 +1415,67 @@ let SUBGROUP_OF_SETWISE = prove
         s SUBSET group_carrier G /\
         group_id G IN s /\
         group_setinv G s SUBSET s /\
-        group_setop G s s SUBSET s`,
-  REWRITE_TAC[subgroup_of; group_setinv; group_setop] THEN SET_TAC[]);;
+        group_setmul G s s SUBSET s`,
+  REWRITE_TAC[subgroup_of; group_setinv; group_setmul] THEN SET_TAC[]);;
 
 let OPPOSITE_GROUP_SETINV = prove
  (`!G s:A->bool.
         group_setinv (opposite_group G) s = group_setinv G s`,
   REPEAT STRIP_TAC THEN REWRITE_TAC[group_setinv; OPPOSITE_GROUP]);;
 
-let OPPOSITE_GROUP_SETOP = prove
+let OPPOSITE_GROUP_SETMUL = prove
  (`!G s t:A->bool.
-        group_setop (opposite_group G) s t = group_setop G t s`,
-  REPEAT STRIP_TAC THEN REWRITE_TAC[group_setop; OPPOSITE_GROUP] THEN
+        group_setmul (opposite_group G) s t = group_setmul G t s`,
+  REPEAT STRIP_TAC THEN REWRITE_TAC[group_setmul; OPPOSITE_GROUP] THEN
   SET_TAC[]);;
 
 let GROUP_SETINV_EQ_EMPTY = prove
  (`!G g:A->bool. group_setinv G g = {} <=> g = {}`,
   REWRITE_TAC[group_setinv] THEN SET_TAC[]);;
 
-let GROUP_SETOP_EQ_EMPTY = prove
- (`!G g h:A->bool. group_setop G g h = {} <=> g = {} \/ h = {}`,
-  REWRITE_TAC[group_setop] THEN SET_TAC[]);;
+let GROUP_SETMUL_EQ_EMPTY = prove
+ (`!G g h:A->bool. group_setmul G g h = {} <=> g = {} \/ h = {}`,
+  REWRITE_TAC[group_setmul] THEN SET_TAC[]);;
 
 let GROUP_SETINV_SING = prove
  (`!G x:A. group_setinv G {x} = {group_inv G x}`,
   REWRITE_TAC[group_setinv] THEN SET_TAC[]);;
 
-let GROUP_SETOP_SING = prove
- (`!G x y:A. group_setop G {x} {y} = {group_op G x y}`,
-  REWRITE_TAC[group_setop] THEN SET_TAC[]);;
+let GROUP_SETMUL_SING = prove
+ (`!G x y:A. group_setmul G {x} {y} = {group_mul G x y}`,
+  REWRITE_TAC[group_setmul] THEN SET_TAC[]);;
 
 let GROUP_SETINV = prove
  (`!G g:A->bool.
         g SUBSET group_carrier G ==> group_setinv G g SUBSET group_carrier G`,
   SIMP_TAC[group_setinv; SUBSET; FORALL_IN_GSPEC; GROUP_INV]);;
 
-let GROUP_SETOP = prove
+let GROUP_SETMUL = prove
  (`!G g h:A->bool.
         g SUBSET group_carrier G /\ h SUBSET group_carrier G==>
-        group_setop G g h SUBSET group_carrier G`,
-  SIMP_TAC[group_setop; SUBSET; FORALL_IN_GSPEC; GROUP_OP]);;
+        group_setmul G g h SUBSET group_carrier G`,
+  SIMP_TAC[group_setmul; SUBSET; FORALL_IN_GSPEC; GROUP_MUL]);;
 
-let GROUP_SETOP_LID = prove
+let GROUP_SETMUL_LID = prove
  (`!G g:A->bool.
-        g SUBSET group_carrier G ==> group_setop G {group_id G} g = g`,
-  REPEAT STRIP_TAC THEN REWRITE_TAC[group_setop] THEN MATCH_MP_TAC(SET_RULE
+        g SUBSET group_carrier G ==> group_setmul G {group_id G} g = g`,
+  REPEAT STRIP_TAC THEN REWRITE_TAC[group_setmul] THEN MATCH_MP_TAC(SET_RULE
    `(!y. y IN s ==> f a y = y) ==> {f x y | x IN {a} /\ y IN s} = s`) THEN
-  RULE_ASSUM_TAC(REWRITE_RULE[SUBSET]) THEN ASM_SIMP_TAC[GROUP_OP_LID]);;
+  RULE_ASSUM_TAC(REWRITE_RULE[SUBSET]) THEN ASM_SIMP_TAC[GROUP_MUL_LID]);;
 
-let GROUP_SETOP_RID = prove
+let GROUP_SETMUL_RID = prove
  (`!G g:A->bool.
-        g SUBSET group_carrier G ==> group_setop G g {group_id G} = g`,
-  ONCE_REWRITE_TAC[GSYM OPPOSITE_GROUP_SETOP] THEN
-  MESON_TAC[GROUP_SETOP_LID; OPPOSITE_GROUP]);;
+        g SUBSET group_carrier G ==> group_setmul G g {group_id G} = g`,
+  ONCE_REWRITE_TAC[GSYM OPPOSITE_GROUP_SETMUL] THEN
+  MESON_TAC[GROUP_SETMUL_LID; OPPOSITE_GROUP]);;
 
-let GROUP_SETOP_ASSOC = prove
+let GROUP_SETMUL_ASSOC = prove
  (`!G g h i:A->bool.
         g SUBSET group_carrier G /\ h SUBSET group_carrier G /\
         i SUBSET group_carrier G
-        ==> group_setop G g (group_setop G h i) =
-            group_setop G (group_setop G g h) i`,
-  REPEAT STRIP_TAC THEN REWRITE_TAC[group_setop] THEN
+        ==> group_setmul G g (group_setmul G h i) =
+            group_setmul G (group_setmul G g h) i`,
+  REPEAT STRIP_TAC THEN REWRITE_TAC[group_setmul] THEN
   REWRITE_TAC[SET_RULE
    `{f x y |x,y| x IN s /\ y IN {g w z | w IN t /\ z IN u}} =
     {f x (g y z) | x IN s /\ y IN t /\ z IN u}`] THEN
@@ -1182,7 +1485,7 @@ let GROUP_SETOP_ASSOC = prove
   MATCH_MP_TAC(SET_RULE
    `(!x y z. P x y z ==> f x y z = g x y z)
     ==> {f x y z | P x y z} = {g x y z | P x y z}`) THEN
-  REPEAT STRIP_TAC THEN MATCH_MP_TAC GROUP_OP_ASSOC THEN
+  REPEAT STRIP_TAC THEN MATCH_MP_TAC GROUP_MUL_ASSOC THEN
   ASM SET_TAC[]);;
 
 let GROUP_SETINV_SUBGROUP = prove
@@ -1192,220 +1495,220 @@ let GROUP_SETINV_SUBGROUP = prove
    `(!x. x IN s ==> f x IN s /\ f(f x) = x) ==> {f x | x IN s} = s`) THEN
   ASM_SIMP_TAC[GROUP_INV_INV]);;
 
-let GROUP_SETOP_LSUBSET = prove
+let GROUP_SETMUL_LSUBSET = prove
  (`!G h s:A->bool.
-        h subgroup_of G /\ s SUBSET h /\ ~(s = {}) ==> group_setop G s h = h`,
-  REWRITE_TAC[group_setop; subgroup_of; SUBSET] THEN REPEAT STRIP_TAC THEN
-  ASM_SIMP_TAC[GSYM SUBSET_ANTISYM_EQ; SUBSET; GROUP_OP; FORALL_IN_GSPEC] THEN
+        h subgroup_of G /\ s SUBSET h /\ ~(s = {}) ==> group_setmul G s h = h`,
+  REWRITE_TAC[group_setmul; subgroup_of; SUBSET] THEN REPEAT STRIP_TAC THEN
+  ASM_SIMP_TAC[GSYM SUBSET_ANTISYM_EQ; SUBSET; GROUP_MUL; FORALL_IN_GSPEC] THEN
   X_GEN_TAC `x:A` THEN DISCH_TAC THEN REWRITE_TAC[IN_ELIM_THM] THEN
   FIRST_X_ASSUM(X_CHOOSE_TAC `y:A` o REWRITE_RULE[GSYM MEMBER_NOT_EMPTY]) THEN
-  MAP_EVERY EXISTS_TAC [`y:A`; `group_op G (group_inv G y) x:A`] THEN
+  MAP_EVERY EXISTS_TAC [`y:A`; `group_mul G (group_inv G y) x:A`] THEN
   ASM_SIMP_TAC[] THEN
-  W(MP_TAC o PART_MATCH (lhand o rand) GROUP_OP_ASSOC o rand o snd) THEN
-  ASM_SIMP_TAC[GROUP_OP; GROUP_INV; GROUP_OP_RINV; GROUP_OP_LID]);;
+  W(MP_TAC o PART_MATCH (lhand o rand) GROUP_MUL_ASSOC o rand o snd) THEN
+  ASM_SIMP_TAC[GROUP_MUL; GROUP_INV; GROUP_MUL_RINV; GROUP_MUL_LID]);;
 
-let GROUP_SETOP_RSUBSET = prove
+let GROUP_SETMUL_RSUBSET = prove
  (`!G h s:A->bool.
-        h subgroup_of G /\ s SUBSET h /\ ~(s = {}) ==> group_setop G h s = h`,
-  ONCE_REWRITE_TAC[GSYM OPPOSITE_GROUP_SETOP] THEN
-  SIMP_TAC[GROUP_SETOP_LSUBSET; SUBGROUP_OF_OPPOSITE_GROUP; OPPOSITE_GROUP]);;
+        h subgroup_of G /\ s SUBSET h /\ ~(s = {}) ==> group_setmul G h s = h`,
+  ONCE_REWRITE_TAC[GSYM OPPOSITE_GROUP_SETMUL] THEN
+  SIMP_TAC[GROUP_SETMUL_LSUBSET; SUBGROUP_OF_OPPOSITE_GROUP; OPPOSITE_GROUP]);;
 
-let GROUP_SETOP_LSUBSET_EQ = prove
+let GROUP_SETMUL_LSUBSET_EQ = prove
  (`!G h s:A->bool.
         h subgroup_of G /\ s SUBSET group_carrier G
-        ==> (group_setop G s h = h <=> s SUBSET h /\ ~(s = {}))`,
+        ==> (group_setmul G s h = h <=> s SUBSET h /\ ~(s = {}))`,
   REPEAT STRIP_TAC THEN ASM_CASES_TAC `s:A->bool = {}` THENL
-   [ASM_MESON_TAC[GROUP_SETOP_EQ_EMPTY; SUBGROUP_OF_IMP_NONEMPTY];
+   [ASM_MESON_TAC[GROUP_SETMUL_EQ_EMPTY; SUBGROUP_OF_IMP_NONEMPTY];
     ASM_REWRITE_TAC[]] THEN
-  EQ_TAC THENL [ALL_TAC; ASM_MESON_TAC[GROUP_SETOP_LSUBSET]] THEN
+  EQ_TAC THENL [ALL_TAC; ASM_MESON_TAC[GROUP_SETMUL_LSUBSET]] THEN
   DISCH_THEN(SUBST1_TAC o SYM) THEN
-  REWRITE_TAC[group_setop; IN_ELIM_THM; SUBSET] THEN
+  REWRITE_TAC[group_setmul; IN_ELIM_THM; SUBSET] THEN
   X_GEN_TAC `x:A` THEN DISCH_TAC THEN
   MAP_EVERY EXISTS_TAC [`x:A`; `group_id G:A`] THEN
   RULE_ASSUM_TAC(REWRITE_RULE[subgroup_of; SUBSET]) THEN
-  ASM_SIMP_TAC[GROUP_OP_RID]);;
+  ASM_SIMP_TAC[GROUP_MUL_RID]);;
 
-let GROUP_SETOP_RSUBSET_EQ = prove
+let GROUP_SETMUL_RSUBSET_EQ = prove
  (`!G h s:A->bool.
         h subgroup_of G /\ s SUBSET group_carrier G
-        ==> (group_setop G h s = h <=> s SUBSET h /\ ~(s = {}))`,
-  ONCE_REWRITE_TAC[GSYM OPPOSITE_GROUP_SETOP] THEN
-  SIMP_TAC[GROUP_SETOP_LSUBSET_EQ; SUBGROUP_OF_OPPOSITE_GROUP;
+        ==> (group_setmul G h s = h <=> s SUBSET h /\ ~(s = {}))`,
+  ONCE_REWRITE_TAC[GSYM OPPOSITE_GROUP_SETMUL] THEN
+  SIMP_TAC[GROUP_SETMUL_LSUBSET_EQ; SUBGROUP_OF_OPPOSITE_GROUP;
            OPPOSITE_GROUP]);;
 
-let GROUP_SETOP_SUBGROUP = prove
+let GROUP_SETMUL_SUBGROUP = prove
  (`!G h:A->bool.
-        h subgroup_of G ==> group_setop G h h = h`,
-  REPEAT STRIP_TAC THEN MATCH_MP_TAC GROUP_SETOP_LSUBSET THEN
+        h subgroup_of G ==> group_setmul G h h = h`,
+  REPEAT STRIP_TAC THEN MATCH_MP_TAC GROUP_SETMUL_LSUBSET THEN
   ASM_MESON_TAC[SUBGROUP_OF_IMP_NONEMPTY; SUBSET_REFL]);;
 
-let GROUP_SETOP_LCANCEL = prove
+let GROUP_SETMUL_LCANCEL = prove
  (`!G g h x:A.
         x IN group_carrier G /\
         g SUBSET group_carrier G /\ h SUBSET group_carrier G
-        ==> (group_setop G {x} g = group_setop G {x} h <=> g = h)`,
+        ==> (group_setmul G {x} g = group_setmul G {x} h <=> g = h)`,
   REPEAT STRIP_TAC THEN EQ_TAC THEN SIMP_TAC[] THEN
-  DISCH_THEN(MP_TAC o AP_TERM `group_setop G {group_inv G x:A}`) THEN
-  ASM_SIMP_TAC[GROUP_SETOP_ASSOC; SING_SUBSET; GROUP_INV] THEN
-  ASM_SIMP_TAC[GROUP_SETOP_SING; GROUP_OP_LINV; GROUP_SETOP_LID]);;
+  DISCH_THEN(MP_TAC o AP_TERM `group_setmul G {group_inv G x:A}`) THEN
+  ASM_SIMP_TAC[GROUP_SETMUL_ASSOC; SING_SUBSET; GROUP_INV] THEN
+  ASM_SIMP_TAC[GROUP_SETMUL_SING; GROUP_MUL_LINV; GROUP_SETMUL_LID]);;
 
-let GROUP_SETOP_RCANCEL = prove
+let GROUP_SETMUL_RCANCEL = prove
  (`!G g h x:A.
         x IN group_carrier G /\ g SUBSET group_carrier G /\
         h SUBSET group_carrier G
-        ==> (group_setop G g {x} = group_setop G h {x} <=> g = h)`,
-  ONCE_REWRITE_TAC[GSYM OPPOSITE_GROUP_SETOP] THEN
-  SIMP_TAC[GROUP_SETOP_LCANCEL; OPPOSITE_GROUP]);;
+        ==> (group_setmul G g {x} = group_setmul G h {x} <=> g = h)`,
+  ONCE_REWRITE_TAC[GSYM OPPOSITE_GROUP_SETMUL] THEN
+  SIMP_TAC[GROUP_SETMUL_LCANCEL; OPPOSITE_GROUP]);;
 
-let GROUP_SETOP_LCANCEL_SET = prove
+let GROUP_SETMUL_LCANCEL_SET = prove
  (`!G h x y:A.
         x IN group_carrier G /\ y IN group_carrier G /\ h subgroup_of G
-        ==> (group_setop G h {x} = group_setop G h {y} <=>
+        ==> (group_setmul G h {x} = group_setmul G h {y} <=>
              group_div G x y IN h)`,
   REPEAT STRIP_TAC THEN
   FIRST_ASSUM(ASSUME_TAC o MATCH_MP SUBGROUP_OF_IMP_SUBSET) THEN
   TRANS_TAC EQ_TRANS
-   `group_setop G (group_setop G h {x}) {group_inv G y}  =
-    group_setop G (group_setop G h {y:A}) {group_inv G y}` THEN
+   `group_setmul G (group_setmul G h {x}) {group_inv G y}  =
+    group_setmul G (group_setmul G h {y:A}) {group_inv G y}` THEN
   CONJ_TAC THENL
-   [CONV_TAC SYM_CONV THEN MATCH_MP_TAC GROUP_SETOP_RCANCEL THEN
-    ASM_SIMP_TAC[GROUP_INV; GROUP_SETOP; SING_SUBSET];
-    ASM_SIMP_TAC[GSYM GROUP_SETOP_ASSOC; GROUP_INV; SING_SUBSET] THEN
-    ASM_SIMP_TAC[GROUP_SETOP_SING; GROUP_OP_RINV; GROUP_SETOP_RID] THEN
-    ASM_SIMP_TAC[GROUP_SETOP_RSUBSET_EQ; SING_SUBSET; group_div;
-                 GROUP_INV; GROUP_OP; NOT_INSERT_EMPTY]]);;
+   [CONV_TAC SYM_CONV THEN MATCH_MP_TAC GROUP_SETMUL_RCANCEL THEN
+    ASM_SIMP_TAC[GROUP_INV; GROUP_SETMUL; SING_SUBSET];
+    ASM_SIMP_TAC[GSYM GROUP_SETMUL_ASSOC; GROUP_INV; SING_SUBSET] THEN
+    ASM_SIMP_TAC[GROUP_SETMUL_SING; GROUP_MUL_RINV; GROUP_SETMUL_RID] THEN
+    ASM_SIMP_TAC[GROUP_SETMUL_RSUBSET_EQ; SING_SUBSET; group_div;
+                 GROUP_INV; GROUP_MUL; NOT_INSERT_EMPTY]]);;
 
-let GROUP_SETOP_RCANCEL_SET = prove
+let GROUP_SETMUL_RCANCEL_SET = prove
  (`!G h x y:A.
         x IN group_carrier G /\ y IN group_carrier G /\ h subgroup_of G
-        ==> (group_setop G {x} h = group_setop G {y} h <=>
-             group_op G (group_inv G x) y IN h)`,
+        ==> (group_setmul G {x} h = group_setmul G {y} h <=>
+             group_mul G (group_inv G x) y IN h)`,
   REPEAT STRIP_TAC THEN GEN_REWRITE_TAC LAND_CONV [EQ_SYM_EQ] THEN
-  ONCE_REWRITE_TAC[GSYM OPPOSITE_GROUP_SETOP] THEN
-  ASM_SIMP_TAC[GROUP_SETOP_LCANCEL_SET; OPPOSITE_GROUP;
+  ONCE_REWRITE_TAC[GSYM OPPOSITE_GROUP_SETMUL] THEN
+  ASM_SIMP_TAC[GROUP_SETMUL_LCANCEL_SET; OPPOSITE_GROUP;
                SUBGROUP_OF_OPPOSITE_GROUP; group_div]);;
 
-let SUBGROUP_SETOP_EQ = prove
+let SUBGROUP_SETMUL_EQ = prove
  (`!G g h:A->bool.
         g subgroup_of G /\ h subgroup_of G
-        ==> ((group_setop G g h) subgroup_of G <=>
-             group_setop G g h = group_setop G h g)`,
+        ==> ((group_setmul G g h) subgroup_of G <=>
+             group_setmul G g h = group_setmul G h g)`,
   REPEAT STRIP_TAC THEN EQ_TAC THENL
    [DISCH_TAC THEN MATCH_MP_TAC SUBSET_ANTISYM THEN
-    REWRITE_TAC[SUBSET; group_setop; FORALL_IN_GSPEC] THEN
+    REWRITE_TAC[SUBSET; group_setmul; FORALL_IN_GSPEC] THEN
     CONJ_TAC THEN MAP_EVERY X_GEN_TAC [`x:A`; `y:A`] THEN STRIP_TAC THEN
     REWRITE_TAC[IN_ELIM_THM] THEN
     FIRST_ASSUM(MP_TAC o GEN_REWRITE_RULE I [subgroup_of]) THEN
     DISCH_THEN(MP_TAC o el 2 o CONJUNCTS) THENL
-     [DISCH_THEN(MP_TAC o SPEC `group_op G x y:A`) THEN
-      REWRITE_TAC[group_setop; IN_ELIM_THM] THEN
+     [DISCH_THEN(MP_TAC o SPEC `group_mul G x y:A`) THEN
+      REWRITE_TAC[group_setmul; IN_ELIM_THM] THEN
       ANTS_TAC THENL [ASM_MESON_TAC[]; REWRITE_TAC[LEFT_IMP_EXISTS_THM]] THEN
       MAP_EVERY X_GEN_TAC [`w:A`; `z:A`] THEN STRIP_TAC THEN
       FIRST_X_ASSUM(MP_TAC o AP_TERM `group_inv (G:A group)`) THEN
       RULE_ASSUM_TAC(REWRITE_RULE[subgroup_of; SUBSET]) THEN
-      ASM_SIMP_TAC[GROUP_INV_INV; GROUP_OP] THEN
-      ASM_SIMP_TAC[GROUP_INV_OP] THEN ASM_MESON_TAC[];
+      ASM_SIMP_TAC[GROUP_INV_INV; GROUP_MUL] THEN
+      ASM_SIMP_TAC[GROUP_INV_MUL] THEN ASM_MESON_TAC[];
       DISCH_THEN(MP_TAC o SPEC
-       `group_op G (group_inv G y) (group_inv G x):A`) THEN
+       `group_mul G (group_inv G y) (group_inv G x):A`) THEN
       RULE_ASSUM_TAC(REWRITE_RULE[subgroup_of; SUBSET]) THEN
-      REWRITE_TAC[group_setop; IN_ELIM_THM] THEN
+      REWRITE_TAC[group_setmul; IN_ELIM_THM] THEN
       ANTS_TAC THENL [ASM_MESON_TAC[]; REWRITE_TAC[LEFT_IMP_EXISTS_THM]] THEN
-      ASM_SIMP_TAC[GROUP_INV_OP; GROUP_INV; GROUP_OP; GROUP_INV_INV] THEN
+      ASM_SIMP_TAC[GROUP_INV_MUL; GROUP_INV; GROUP_MUL; GROUP_INV_INV] THEN
       ASM_MESON_TAC[]];
     DISCH_TAC THEN REWRITE_TAC[SUBGROUP_OF_SETWISE] THEN
-    ASM_SIMP_TAC[GROUP_SETOP; SUBGROUP_OF_IMP_SUBSET] THEN
+    ASM_SIMP_TAC[GROUP_SETMUL; SUBGROUP_OF_IMP_SUBSET] THEN
     REWRITE_TAC[CONJ_ASSOC] THEN CONJ_TAC THENL
-     [REWRITE_TAC[group_setop; group_setinv; SUBSET; IMP_CONJ;
+     [REWRITE_TAC[group_setmul; group_setinv; SUBSET; IMP_CONJ;
                   RIGHT_FORALL_IMP_THM; FORALL_IN_GSPEC] THEN
       RULE_ASSUM_TAC(REWRITE_RULE[subgroup_of; SUBSET]) THEN
-      ASM_SIMP_TAC[GROUP_INV_OP; IN_ELIM_THM] THEN
-      CONJ_TAC THENL [ASM_MESON_TAC[GROUP_OP_LID]; ALL_TAC] THEN
+      ASM_SIMP_TAC[GROUP_INV_MUL; IN_ELIM_THM] THEN
+      CONJ_TAC THENL [ASM_MESON_TAC[GROUP_MUL_LID]; ALL_TAC] THEN
       X_GEN_TAC `y:A` THEN DISCH_TAC THEN X_GEN_TAC `x:A` THEN DISCH_TAC THEN
       FIRST_X_ASSUM(MP_TAC o MATCH_MP(SET_RULE
        `s = t ==> !x. x IN s ==> x IN t`)) THEN
-      REWRITE_TAC[group_setop; FORALL_IN_GSPEC] THEN
+      REWRITE_TAC[group_setmul; FORALL_IN_GSPEC] THEN
       DISCH_THEN(MP_TAC o SPECL [`group_inv G x:A`; `group_inv G y:A`]) THEN
       ASM SET_TAC[];
       TRANS_TAC SUBSET_TRANS
-       `group_setop G (group_setop G h g) (group_setop G g h):A->bool` THEN
+       `group_setmul G (group_setmul G h g) (group_setmul G g h):A->bool` THEN
       CONJ_TAC THENL [ASM_MESON_TAC[SUBSET_REFL]; ALL_TAC] THEN
       TRANS_TAC SUBSET_TRANS
-       `group_setop G h (group_setop G g (group_setop G g h)):A->bool` THEN
+       `group_setmul G h (group_setmul G g (group_setmul G g h)):A->bool` THEN
       CONJ_TAC THENL
-       [ASM_MESON_TAC[GROUP_SETOP_ASSOC; subgroup_of; GROUP_SETOP;
+       [ASM_MESON_TAC[GROUP_SETMUL_ASSOC; subgroup_of; GROUP_SETMUL;
                       SUBSET_REFL];
         ALL_TAC] THEN
       TRANS_TAC SUBSET_TRANS
-       `group_setop G h (group_setop G (group_setop G g g) h):A->bool` THEN
+       `group_setmul G h (group_setmul G (group_setmul G g g) h):A->bool` THEN
       CONJ_TAC THENL
-       [ASM_MESON_TAC[GROUP_SETOP_ASSOC; subgroup_of; GROUP_SETOP;
+       [ASM_MESON_TAC[GROUP_SETMUL_ASSOC; subgroup_of; GROUP_SETMUL;
                       SUBSET_REFL];
         ALL_TAC] THEN
-      ASM_SIMP_TAC[GROUP_SETOP_SUBGROUP] THEN
-      ASM_SIMP_TAC[GROUP_SETOP_ASSOC; SUBGROUP_OF_IMP_SUBSET] THEN
-      ASM_SIMP_TAC[GROUP_SETOP_SUBGROUP; SUBSET_REFL]]]);;
+      ASM_SIMP_TAC[GROUP_SETMUL_SUBGROUP] THEN
+      ASM_SIMP_TAC[GROUP_SETMUL_ASSOC; SUBGROUP_OF_IMP_SUBSET] THEN
+      ASM_SIMP_TAC[GROUP_SETMUL_SUBGROUP; SUBSET_REFL]]]);;
 
 let SUBGROUP_GENERATED_SETOP = prove
  (`!G g h:A->bool.
         g subgroup_of G /\ h subgroup_of G
-        ==> subgroup_generated G (group_setop G g h) =
+        ==> subgroup_generated G (group_setmul G g h) =
             subgroup_generated G (g UNION h)`,
   REPEAT STRIP_TAC THEN
   REWRITE_TAC[GROUPS_EQ; CONJUNCT2 SUBGROUP_GENERATED] THEN
   MATCH_MP_TAC SUBSET_ANTISYM THEN CONJ_TAC THEN
   MATCH_MP_TAC SUBGROUP_GENERATED_MINIMAL THEN
   REWRITE_TAC[SUBGROUP_SUBGROUP_GENERATED] THEN
-  REWRITE_TAC[SUBSET; group_setop; FORALL_IN_GSPEC; FORALL_IN_UNION] THENL
-   [REPEAT STRIP_TAC THEN MATCH_MP_TAC(MESON[SUBGROUP_GENERATED; GROUP_OP]
+  REWRITE_TAC[SUBSET; group_setmul; FORALL_IN_GSPEC; FORALL_IN_UNION] THENL
+   [REPEAT STRIP_TAC THEN MATCH_MP_TAC(MESON[SUBGROUP_GENERATED; GROUP_MUL]
      `x IN group_carrier(subgroup_generated G s) /\
       y IN group_carrier(subgroup_generated G s)
-      ==> group_op G x y IN group_carrier(subgroup_generated G s)`) THEN
+      ==> group_mul G x y IN group_carrier(subgroup_generated G s)`) THEN
     CONJ_TAC;
     REPEAT STRIP_TAC] THEN
   MATCH_MP_TAC SUBGROUP_GENERATED_INC THEN
   ASM_SIMP_TAC[UNION_SUBSET; IN_UNION; SUBGROUP_OF_IMP_SUBSET] THEN
-  ASM_SIMP_TAC[GSYM group_setop; GROUP_SETOP; SUBGROUP_OF_IMP_SUBSET] THEN
-  REWRITE_TAC[group_setop; IN_ELIM_THM] THEN
-  ASM_MESON_TAC[GROUP_OP_LID; GROUP_OP_RID; subgroup_of; SUBSET]);;
+  ASM_SIMP_TAC[GSYM group_setmul; GROUP_SETMUL; SUBGROUP_OF_IMP_SUBSET] THEN
+  REWRITE_TAC[group_setmul; IN_ELIM_THM] THEN
+  ASM_MESON_TAC[GROUP_MUL_LID; GROUP_MUL_RID; subgroup_of; SUBSET]);;
 
 (* ------------------------------------------------------------------------- *)
 (* Right and left cosets.                                                    *)
 (* ------------------------------------------------------------------------- *)
 
 let right_coset = new_definition
- `right_coset G h x = group_setop G h {x}`;;
+ `right_coset G h x = group_setmul G h {x}`;;
 
 let left_coset = new_definition
- `left_coset G x h = group_setop G {x} h`;;
+ `left_coset G x h = group_setmul G {x} h`;;
 
 let RIGHT_COSET = prove
  (`!G h x:A.
         x IN group_carrier G /\ h SUBSET group_carrier G
         ==> right_coset G h x SUBSET group_carrier G`,
-  SIMP_TAC[right_coset; GROUP_SETOP; SING_SUBSET]);;
+  SIMP_TAC[right_coset; GROUP_SETMUL; SING_SUBSET]);;
 
 let LEFT_COSET = prove
  (`!G h x:A.
         x IN group_carrier G /\ h SUBSET group_carrier G
         ==> left_coset G x h SUBSET group_carrier G`,
-  SIMP_TAC[left_coset; GROUP_SETOP; SING_SUBSET]);;
+  SIMP_TAC[left_coset; GROUP_SETMUL; SING_SUBSET]);;
 
 let RIGHT_COSET_OPPOSITE_GROUP = prove
  (`!G h x:A. right_coset G h x = left_coset (opposite_group G) x h`,
-  REWRITE_TAC[left_coset; right_coset; OPPOSITE_GROUP_SETOP]);;
+  REWRITE_TAC[left_coset; right_coset; OPPOSITE_GROUP_SETMUL]);;
 
 let LEFT_COSET_OPPOSITE_GROUP = prove
  (`!G h x:A. left_coset G x h = right_coset (opposite_group G) h x`,
-  REWRITE_TAC[left_coset; right_coset; OPPOSITE_GROUP_SETOP]);;
+  REWRITE_TAC[left_coset; right_coset; OPPOSITE_GROUP_SETMUL]);;
 
 let RIGHT_COSET_ID = prove
  (`!G h:A->bool.
         h SUBSET group_carrier G ==> right_coset G h (group_id G) = h`,
-  SIMP_TAC[right_coset; group_setop; SET_RULE
+  SIMP_TAC[right_coset; group_setmul; SET_RULE
    `{f x y | P x /\ y IN {a}} = {f x a | P x}`] THEN
   REWRITE_TAC[SUBSET] THEN REPEAT STRIP_TAC THEN MATCH_MP_TAC(SET_RULE
    `(!x. x IN s ==> f x = x) ==> {f x | x IN s} = s`) THEN
-  ASM_SIMP_TAC[GROUP_OP_RID]);;
+  ASM_SIMP_TAC[GROUP_MUL_RID]);;
 
 let LEFT_COSET_ID = prove
  (`!G h:A->bool.
@@ -1414,58 +1717,58 @@ let LEFT_COSET_ID = prove
 
 let LEFT_COSET_TRIVIAL = prove
  (`!G x:A. x IN group_carrier G ==> left_coset G x {group_id G} = {x}`,
-  SIMP_TAC[left_coset; GROUP_SETOP_SING; GROUP_ID; GROUP_OP_RID]);;
+  SIMP_TAC[left_coset; GROUP_SETMUL_SING; GROUP_ID; GROUP_MUL_RID]);;
 
 let RIGHT_COSET_TRIVIAL = prove
  (`!G x:A. x IN group_carrier G ==> right_coset G {group_id G} x = {x}`,
-  SIMP_TAC[right_coset; GROUP_SETOP_SING; GROUP_ID; GROUP_OP_LID]);;
+  SIMP_TAC[right_coset; GROUP_SETMUL_SING; GROUP_ID; GROUP_MUL_LID]);;
 
 let LEFT_COSET_CARRIER = prove
  (`!G x:A. x IN group_carrier G
            ==> left_coset G x (group_carrier G) = group_carrier G`,
-  SIMP_TAC[left_coset; GROUP_SETOP_LSUBSET; SING_SUBSET; NOT_INSERT_EMPTY;
+  SIMP_TAC[left_coset; GROUP_SETMUL_LSUBSET; SING_SUBSET; NOT_INSERT_EMPTY;
            CARRIER_SUBGROUP_OF]);;
 
 let RIGHT_COSET_CARRIER = prove
  (`!G x:A. x IN group_carrier G
            ==> right_coset G (group_carrier G) x = group_carrier G`,
-  SIMP_TAC[right_coset; GROUP_SETOP_RSUBSET; SING_SUBSET; NOT_INSERT_EMPTY;
+  SIMP_TAC[right_coset; GROUP_SETMUL_RSUBSET; SING_SUBSET; NOT_INSERT_EMPTY;
            CARRIER_SUBGROUP_OF]);;
 
 let RIGHT_COSET_EQ = prove
  (`!G h x y:A.
         h subgroup_of G /\ x IN group_carrier G /\ y IN group_carrier G
         ==> (right_coset G h x = right_coset G h y <=> group_div G x y IN h)`,
-  SIMP_TAC[GROUP_SETOP_LCANCEL_SET; right_coset]);;
+  SIMP_TAC[GROUP_SETMUL_LCANCEL_SET; right_coset]);;
 
 let LEFT_COSET_EQ = prove
  (`!G h x y:A.
         h subgroup_of G /\ x IN group_carrier G /\ y IN group_carrier G
         ==> (left_coset G x h = left_coset G y h <=>
-             group_op G (group_inv G x) y IN h)`,
-  SIMP_TAC[GROUP_SETOP_RCANCEL_SET; left_coset]);;
+             group_mul G (group_inv G x) y IN h)`,
+  SIMP_TAC[GROUP_SETMUL_RCANCEL_SET; left_coset]);;
 
 let RIGHT_COSET_EQ_SUBGROUP = prove
  (`!G h x:A.
         h subgroup_of G /\ x IN group_carrier G
         ==> (right_coset G h x = h <=> x IN h)`,
-  SIMP_TAC[right_coset; GROUP_SETOP_RSUBSET_EQ; SING_SUBSET] THEN
+  SIMP_TAC[right_coset; GROUP_SETMUL_RSUBSET_EQ; SING_SUBSET] THEN
   REWRITE_TAC[NOT_INSERT_EMPTY]);;
 
 let LEFT_COSET_EQ_SUBGROUP = prove
  (`!G h x:A.
         h subgroup_of G /\ x IN group_carrier G
         ==> (left_coset G x h = h <=> x IN h)`,
-  SIMP_TAC[left_coset; GROUP_SETOP_LSUBSET_EQ; SING_SUBSET] THEN
+  SIMP_TAC[left_coset; GROUP_SETMUL_LSUBSET_EQ; SING_SUBSET] THEN
   REWRITE_TAC[NOT_INSERT_EMPTY]);;
 
 let RIGHT_COSET_EQ_EMPTY = prove
  (`!G h x:A. right_coset G h x = {} <=> h = {}`,
-  REWRITE_TAC[right_coset; GROUP_SETOP_EQ_EMPTY; NOT_INSERT_EMPTY]);;
+  REWRITE_TAC[right_coset; GROUP_SETMUL_EQ_EMPTY; NOT_INSERT_EMPTY]);;
 
 let LEFT_COSET_EQ_EMPTY = prove
  (`!G h x:A. left_coset G x h = {} <=> h = {}`,
-  REWRITE_TAC[left_coset; GROUP_SETOP_EQ_EMPTY; NOT_INSERT_EMPTY]);;
+  REWRITE_TAC[left_coset; GROUP_SETMUL_EQ_EMPTY; NOT_INSERT_EMPTY]);;
 
 let RIGHT_COSET_NONEMPTY = prove
  (`!G h x:A. h subgroup_of G ==> ~(right_coset G h x = {})`,
@@ -1478,14 +1781,14 @@ let LEFT_COSET_NONEMPTY = prove
 let IN_RIGHT_COSET_SELF = prove
  (`!G h x:A.
       h subgroup_of G /\ x IN group_carrier G ==> x IN right_coset G h x`,
-  REWRITE_TAC[subgroup_of; right_coset; group_setop; IN_ELIM_THM; IN_SING] THEN
-  MESON_TAC[GROUP_OP_LID]);;
+  REWRITE_TAC[subgroup_of; right_coset; group_setmul; IN_ELIM_THM; IN_SING] THEN
+  MESON_TAC[GROUP_MUL_LID]);;
 
 let IN_LEFT_COSET_SELF = prove
  (`!G h x:A.
       h subgroup_of G /\ x IN group_carrier G ==> x IN left_coset G x h`,
-  REWRITE_TAC[subgroup_of; left_coset; group_setop; IN_ELIM_THM; IN_SING] THEN
-  MESON_TAC[GROUP_OP_RID]);;
+  REWRITE_TAC[subgroup_of; left_coset; group_setmul; IN_ELIM_THM; IN_SING] THEN
+  MESON_TAC[GROUP_MUL_RID]);;
 
 let UNIONS_RIGHT_COSETS = prove
  (`!G h:A->bool.
@@ -1518,15 +1821,15 @@ let RIGHT_COSETS_EQ = prove
   ASM_SIMP_TAC[GSYM DISJOINT_EMPTY_REFL; RIGHT_COSET_NONEMPTY] THEN
   ASM_SIMP_TAC[RIGHT_COSET_EQ; LEFT_IMP_EXISTS_THM; IMP_CONJ; SET_RULE
    `~DISJOINT s t <=> ?x. x IN s /\ ?y. y IN t /\ x = y`] THEN
-  REWRITE_TAC[right_coset; group_setop; FORALL_IN_GSPEC; IN_SING] THEN
+  REWRITE_TAC[right_coset; group_setmul; FORALL_IN_GSPEC; IN_SING] THEN
   REWRITE_TAC[IMP_CONJ; RIGHT_FORALL_IMP_THM; FORALL_UNWIND_THM2] THEN
   X_GEN_TAC `u:A` THEN DISCH_TAC THEN X_GEN_TAC `v:A` THEN DISCH_TAC THEN
-  DISCH_THEN(MP_TAC o AP_TERM `group_op G (group_inv G u):A->A`) THEN
+  DISCH_THEN(MP_TAC o AP_TERM `group_mul G (group_inv G u):A->A`) THEN
   RULE_ASSUM_TAC(REWRITE_RULE[subgroup_of; SUBSET]) THEN
-  ASM_SIMP_TAC[GROUP_OP_ASSOC; GROUP_INV; GROUP_OP_LINV; GROUP_OP_LID] THEN
+  ASM_SIMP_TAC[GROUP_MUL_ASSOC; GROUP_INV; GROUP_MUL_LINV; GROUP_MUL_LID] THEN
   DISCH_THEN SUBST1_TAC THEN
-  ASM_SIMP_TAC[group_div; GSYM GROUP_OP_ASSOC; GROUP_INV; GROUP_OP;
-               GROUP_OP_RINV; GROUP_OP_RID]);;
+  ASM_SIMP_TAC[group_div; GSYM GROUP_MUL_ASSOC; GROUP_INV; GROUP_MUL;
+               GROUP_MUL_RINV; GROUP_MUL_RID]);;
 
 let LEFT_COSETS_EQ = prove
  (`!G h x y:A.
@@ -1553,32 +1856,32 @@ let DISJOINT_LEFT_COSETS = prove
 let IMAGE_RIGHT_COSET_SWITCH = prove
  (`!G h x y:A.
         h subgroup_of G /\ x IN group_carrier G /\ y IN group_carrier G
-        ==> IMAGE (\a. group_op G a (group_op G (group_inv G x) y))
+        ==> IMAGE (\a. group_mul G a (group_mul G (group_inv G x) y))
                   (right_coset G h x) =
             right_coset G h y`,
   REPEAT STRIP_TAC THEN TRANS_TAC EQ_TRANS
-   `group_setop G (right_coset G h x) {group_op G (group_inv G x) y:A}` THEN
-  CONJ_TAC THENL [REWRITE_TAC[group_setop] THEN SET_TAC[]; ALL_TAC] THEN
+   `group_setmul G (right_coset G h x) {group_mul G (group_inv G x) y:A}` THEN
+  CONJ_TAC THENL [REWRITE_TAC[group_setmul] THEN SET_TAC[]; ALL_TAC] THEN
   FIRST_ASSUM(ASSUME_TAC o MATCH_MP SUBGROUP_OF_IMP_SUBSET) THEN
   REWRITE_TAC[right_coset] THEN
-  ASM_SIMP_TAC[GSYM GROUP_SETOP_ASSOC; GROUP_SETOP; SING_SUBSET;
-               GROUP_OP; GROUP_INV; GROUP_SETOP_SING; GROUP_OP_ASSOC;
-               GROUP_OP_RINV; GROUP_OP_LID]);;
+  ASM_SIMP_TAC[GSYM GROUP_SETMUL_ASSOC; GROUP_SETMUL; SING_SUBSET;
+               GROUP_MUL; GROUP_INV; GROUP_SETMUL_SING; GROUP_MUL_ASSOC;
+               GROUP_MUL_RINV; GROUP_MUL_LID]);;
 
 let IMAGE_LEFT_COSET_SWITCH = prove
  (`!G h x y:A.
         h subgroup_of G /\ x IN group_carrier G /\ y IN group_carrier G
-        ==> IMAGE (\a. group_op G (group_div G y x) a)
+        ==> IMAGE (\a. group_mul G (group_div G y x) a)
                   (left_coset G x h) =
             left_coset G y h`,
   REPEAT STRIP_TAC THEN TRANS_TAC EQ_TRANS
-   `group_setop G {group_div G y x:A} (left_coset G x h)` THEN
-  CONJ_TAC THENL [REWRITE_TAC[group_setop] THEN SET_TAC[]; ALL_TAC] THEN
+   `group_setmul G {group_div G y x:A} (left_coset G x h)` THEN
+  CONJ_TAC THENL [REWRITE_TAC[group_setmul] THEN SET_TAC[]; ALL_TAC] THEN
   FIRST_ASSUM(ASSUME_TAC o MATCH_MP SUBGROUP_OF_IMP_SUBSET) THEN
   REWRITE_TAC[left_coset; group_div] THEN
-  ASM_SIMP_TAC[GROUP_SETOP_ASSOC; GROUP_SETOP; SING_SUBSET;
-               GROUP_OP; GROUP_INV; GROUP_SETOP_SING; GSYM GROUP_OP_ASSOC;
-               GROUP_OP_LINV; GROUP_OP_RID]);;
+  ASM_SIMP_TAC[GROUP_SETMUL_ASSOC; GROUP_SETMUL; SING_SUBSET;
+               GROUP_MUL; GROUP_INV; GROUP_SETMUL_SING; GSYM GROUP_MUL_ASSOC;
+               GROUP_MUL_LINV; GROUP_MUL_RID]);;
 
 let CARD_EQ_RIGHT_COSETS = prove
  (`!G h x y:A.
@@ -1591,11 +1894,11 @@ let CARD_EQ_RIGHT_COSETS = prove
     REWRITE_TAC[eq_c; LEFT_FORALL_IMP_THM] THEN
     MATCH_MP_TAC MONO_EXISTS THEN SET_TAC[]) in
   REPEAT STRIP_TAC THEN MATCH_MP_TAC lemma THEN
-  EXISTS_TAC `\a:A. group_op G a (group_op G (group_inv G x) y)` THEN
-  EXISTS_TAC `\a:A. group_op G a (group_op G (group_inv G y) x)` THEN
+  EXISTS_TAC `\a:A. group_mul G a (group_mul G (group_inv G x) y)` THEN
+  EXISTS_TAC `\a:A. group_mul G a (group_mul G (group_inv G y) x)` THEN
   ASM_SIMP_TAC[IMAGE_RIGHT_COSET_SWITCH; INJECTIVE_ON_ALT] THEN
-  REPEAT STRIP_TAC THEN MATCH_MP_TAC GROUP_OP_RCANCEL THEN
-  ASM_MESON_TAC[GROUP_OP; GROUP_INV; SUBSET; RIGHT_COSET;
+  REPEAT STRIP_TAC THEN MATCH_MP_TAC GROUP_MUL_RCANCEL THEN
+  ASM_MESON_TAC[GROUP_MUL; GROUP_INV; SUBSET; RIGHT_COSET;
                 SUBGROUP_OF_IMP_SUBSET]);;
 
 let CARD_EQ_LEFT_COSETS = prove
@@ -1633,7 +1936,7 @@ let LAGRANGE_THEOREM_RIGHT = prove
   ASM_REWRITE_TAC[SIMPLE_IMAGE; IMP_CONJ; RIGHT_FORALL_IMP_THM] THEN
   ASM_SIMP_TAC[FORALL_IN_IMAGE; FINITE_IMAGE] THEN
   ASM_SIMP_TAC[GSYM DISJOINT; DISJOINT_RIGHT_COSETS] THEN
-  REWRITE_TAC[right_coset; group_setop; SET_RULE
+  REWRITE_TAC[right_coset; group_setmul; SET_RULE
    `{f x y | x IN s /\ y IN {a}} = IMAGE (\x. f x a) s`] THEN
   ASM_SIMP_TAC[FINITE_IMAGE] THEN DISCH_THEN SUBST1_TAC THEN
   ASM_SIMP_TAC[GSYM NSUM_CONST; FINITE_IMAGE] THEN
@@ -1641,7 +1944,7 @@ let LAGRANGE_THEOREM_RIGHT = prove
   REPEAT STRIP_TAC THEN CONV_TAC SYM_CONV THEN
   MATCH_MP_TAC CARD_IMAGE_INJ THEN
   RULE_ASSUM_TAC(REWRITE_RULE[subgroup_of; SUBSET]) THEN
-  ASM_SIMP_TAC[IMP_CONJ; GROUP_OP_RCANCEL]);;
+  ASM_SIMP_TAC[IMP_CONJ; GROUP_MUL_RCANCEL]);;
 
 let LAGRANGE_THEOREM_LEFT = prove
  (`!G h:A->bool.
@@ -1689,7 +1992,7 @@ let NORMAL_SUBGROUP_CONJUGATE_ALT = prove
         n normal_subgroup_of G <=>
         n subgroup_of G /\
         !x. x IN group_carrier G
-            ==> group_setop G {group_inv G x} (group_setop G n {x}) = n`,
+            ==> group_setmul G {group_inv G x} (group_setmul G n {x}) = n`,
   REPEAT GEN_TAC THEN REWRITE_TAC[normal_subgroup_of] THEN
   ASM_CASES_TAC `(n:A->bool) subgroup_of G` THEN ASM_REWRITE_TAC[] THEN
   FIRST_ASSUM(ASSUME_TAC o MATCH_MP SUBGROUP_OF_IMP_SUBSET) THEN
@@ -1697,18 +2000,18 @@ let NORMAL_SUBGROUP_CONJUGATE_ALT = prove
   FIRST_X_ASSUM(MP_TAC o SPEC `x:A`) THEN
   ASM_REWRITE_TAC[left_coset; right_coset] THENL
    [DISCH_THEN(SUBST1_TAC o SYM) THEN
-    ASM_SIMP_TAC[GROUP_SETOP_ASSOC; SING_SUBSET; GROUP_INV] THEN
-    ASM_SIMP_TAC[GROUP_SETOP_SING; GROUP_OP_LINV; GROUP_SETOP_LID];
-    DISCH_THEN(MP_TAC o AP_TERM `group_setop G {x:A}`) THEN
-    ASM_SIMP_TAC[GROUP_SETOP_ASSOC; GROUP_INV; GROUP_SETOP; SING_SUBSET] THEN
-    ASM_SIMP_TAC[GROUP_SETOP_SING; GROUP_OP_RINV; GROUP_SETOP_LID]]);;
+    ASM_SIMP_TAC[GROUP_SETMUL_ASSOC; SING_SUBSET; GROUP_INV] THEN
+    ASM_SIMP_TAC[GROUP_SETMUL_SING; GROUP_MUL_LINV; GROUP_SETMUL_LID];
+    DISCH_THEN(MP_TAC o AP_TERM `group_setmul G {x:A}`) THEN
+    ASM_SIMP_TAC[GROUP_SETMUL_ASSOC; GROUP_INV; GROUP_SETMUL; SING_SUBSET] THEN
+    ASM_SIMP_TAC[GROUP_SETMUL_SING; GROUP_MUL_RINV; GROUP_SETMUL_LID]]);;
 
 let NORMAL_SUBGROUP_CONJUGATE = prove
  (`!G n:A->bool.
       n normal_subgroup_of G <=>
       n subgroup_of G /\
       !x. x IN group_carrier G
-          ==> group_setop G {group_inv G x} (group_setop G n {x}) SUBSET n`,
+          ==> group_setmul G {group_inv G x} (group_setmul G n {x}) SUBSET n`,
   REPEAT GEN_TAC THEN REWRITE_TAC[NORMAL_SUBGROUP_CONJUGATE_ALT] THEN
   ASM_CASES_TAC `(n:A->bool) subgroup_of G` THEN ASM_REWRITE_TAC[] THEN
   FIRST_ASSUM(ASSUME_TAC o MATCH_MP SUBGROUP_OF_IMP_SUBSET) THEN
@@ -1716,20 +2019,20 @@ let NORMAL_SUBGROUP_CONJUGATE = prove
   DISCH_TAC THEN X_GEN_TAC `x:A` THEN DISCH_TAC THEN
   FIRST_X_ASSUM(MP_TAC o SPEC `group_inv G (x:A)`) THEN
   ASM_SIMP_TAC[GROUP_INV; GROUP_INV_INV] THEN DISCH_THEN(MP_TAC o
-   ISPEC `\y:A. group_op G (group_inv G x) (group_op G y x)` o
+   ISPEC `\y:A. group_mul G (group_inv G x) (group_mul G y x)` o
    MATCH_MP IMAGE_SUBSET) THEN
-  REWRITE_TAC[group_setop; SIMPLE_IMAGE;
+  REWRITE_TAC[group_setmul; SIMPLE_IMAGE;
     SET_RULE `{f x y | x IN {a} /\ P y} = {f a y | P y}`;
     SET_RULE `{f x y | P x /\ y IN {a}} = {f x a | P x}`] THEN
   REWRITE_TAC[GSYM IMAGE_o; o_DEF] THEN MATCH_MP_TAC(SET_RULE
    `(!x. x IN s ==> f x = x) ==> IMAGE f s SUBSET t ==> s SUBSET t`) THEN
   RULE_ASSUM_TAC(REWRITE_RULE[SUBSET]) THEN
   ASM (CONV_TAC o GEN_SIMPLIFY_CONV TOP_DEPTH_SQCONV (basic_ss []) 4)
-   [GROUP_OP_ASSOC; GROUP_OP; GROUP_INV; GROUP_OP_LINV] THEN
-  ASM_SIMP_TAC[GSYM GROUP_OP_ASSOC; GROUP_OP_LINV; GROUP_OP; GROUP_INV] THEN
-  ASM_SIMP_TAC[GROUP_OP_LID] THEN
-  ASM_SIMP_TAC[GSYM GROUP_OP_ASSOC; GROUP_OP_LINV; GROUP_OP; GROUP_INV] THEN
-  ASM_SIMP_TAC[GROUP_OP_RID]);;
+   [GROUP_MUL_ASSOC; GROUP_MUL; GROUP_INV; GROUP_MUL_LINV] THEN
+  ASM_SIMP_TAC[GSYM GROUP_MUL_ASSOC; GROUP_MUL_LINV; GROUP_MUL; GROUP_INV] THEN
+  ASM_SIMP_TAC[GROUP_MUL_LID] THEN
+  ASM_SIMP_TAC[GSYM GROUP_MUL_ASSOC; GROUP_MUL_LINV; GROUP_MUL; GROUP_INV] THEN
+  ASM_SIMP_TAC[GROUP_MUL_RID]);;
 
 let TRIVIAL_NORMAL_SUBGROUP_OF = prove
  (`!G:A group. {group_id G} normal_subgroup_of G`,
@@ -1750,15 +2053,15 @@ let GROUP_SETINV_RIGHT_COSET = prove
   REPEAT STRIP_TAC THEN
   FIRST_ASSUM(ASSUME_TAC o MATCH_MP SUBGROUP_OF_IMP_SUBSET) THEN
   TRANS_TAC EQ_TRANS
-    `group_setop G {group_inv G a} (group_setinv G n):A->bool` THEN
+    `group_setmul G {group_inv G a} (group_setinv G n):A->bool` THEN
   CONJ_TAC THENL
-   [REWRITE_TAC[group_setinv; group_setop;
+   [REWRITE_TAC[group_setinv; group_setmul;
       SET_RULE `{f x y | P x /\ y IN {a}} = {f x a | P x}`;
       SET_RULE `{f x y | x IN {a} /\ P y} = {f a y | P y}`] THEN
     REWRITE_TAC[SIMPLE_IMAGE; GSYM IMAGE_o] THEN MATCH_MP_TAC(SET_RULE
      `(!x. x IN s ==> f x = g x) ==> IMAGE f s = IMAGE g s`) THEN
     RULE_ASSUM_TAC(REWRITE_RULE[SUBSET]) THEN
-    ASM_SIMP_TAC[GROUP_INV_OP; o_DEF];
+    ASM_SIMP_TAC[GROUP_INV_MUL; o_DEF];
     ASM_SIMP_TAC[GROUP_SETINV_SUBGROUP; GROUP_INV]]);;
 
 let GROUP_SETINV_LEFT_COSET = prove
@@ -1771,37 +2074,37 @@ let GROUP_SETINV_LEFT_COSET = prove
   SIMP_TAC[GROUP_SETINV_RIGHT_COSET; NORMAL_SUBGROUP_OF_OPPOSITE_GROUP;
            OPPOSITE_GROUP]);;
 
-let GROUP_SETOP_RIGHT_COSET = prove
+let GROUP_SETMUL_RIGHT_COSET = prove
  (`!G n a b:A.
         n normal_subgroup_of G /\ a IN group_carrier G /\ b IN group_carrier G
-        ==> group_setop G (right_coset G n a) (right_coset G n b) =
-            right_coset G n (group_op G a b)`,
+        ==> group_setmul G (right_coset G n a) (right_coset G n b) =
+            right_coset G n (group_mul G a b)`,
   REWRITE_TAC[normal_subgroup_of; left_coset; right_coset] THEN
   REPEAT STRIP_TAC THEN
   FIRST_ASSUM(ASSUME_TAC o MATCH_MP SUBGROUP_OF_IMP_SUBSET) THEN
   FIRST_ASSUM(MP_TAC o SPEC `a:A`) THEN
   ANTS_TAC THENL [ASM_REWRITE_TAC[]; DISCH_THEN(SUBST1_TAC o SYM)] THEN
   ASM_SIMP_TAC[SING_SUBSET;
-    MESON[GROUP_SETOP_ASSOC; GROUP_SETOP; GROUP_SETINV]
+    MESON[GROUP_SETMUL_ASSOC; GROUP_SETMUL; GROUP_SETINV]
    `a SUBSET group_carrier G /\ b SUBSET group_carrier G /\
     c SUBSET group_carrier G /\ d SUBSET group_carrier G
-    ==> group_setop G (group_setop G a b) (group_setop G c d) =
-        group_setop G a (group_setop G (group_setop G b c) d)`] THEN
-  ASM_SIMP_TAC[GROUP_SETOP_SUBGROUP] THEN
+    ==> group_setmul G (group_setmul G a b) (group_setmul G c d) =
+        group_setmul G a (group_setmul G (group_setmul G b c) d)`] THEN
+  ASM_SIMP_TAC[GROUP_SETMUL_SUBGROUP] THEN
   FIRST_ASSUM(MP_TAC o SPEC `b:A`) THEN
   ANTS_TAC THENL [ASM_REWRITE_TAC[]; DISCH_THEN(SUBST1_TAC o SYM)] THEN
-  FIRST_X_ASSUM(MP_TAC o SPEC `group_op G a b:A`) THEN
-  ASM_SIMP_TAC[GROUP_OP] THEN DISCH_THEN(SUBST1_TAC o SYM) THEN
-  ASM_SIMP_TAC[GROUP_SETOP_ASSOC; SING_SUBSET; GROUP_SETOP_SING]);;
+  FIRST_X_ASSUM(MP_TAC o SPEC `group_mul G a b:A`) THEN
+  ASM_SIMP_TAC[GROUP_MUL] THEN DISCH_THEN(SUBST1_TAC o SYM) THEN
+  ASM_SIMP_TAC[GROUP_SETMUL_ASSOC; SING_SUBSET; GROUP_SETMUL_SING]);;
 
-let GROUP_SETOP_LEFT_COSET = prove
+let GROUP_SETMUL_LEFT_COSET = prove
  (`!G n a b:A.
         n normal_subgroup_of G /\ a IN group_carrier G /\ b IN group_carrier G
-        ==> group_setop G (left_coset G a n) (left_coset G b n) =
-            left_coset G (group_op G a b) n`,
+        ==> group_setmul G (left_coset G a n) (left_coset G b n) =
+            left_coset G (group_mul G a b) n`,
   REWRITE_TAC[LEFT_COSET_OPPOSITE_GROUP] THEN
-  ONCE_REWRITE_TAC[GSYM OPPOSITE_GROUP_SETOP] THEN
-  SIMP_TAC[GROUP_SETOP_RIGHT_COSET; NORMAL_SUBGROUP_OF_OPPOSITE_GROUP;
+  ONCE_REWRITE_TAC[GSYM OPPOSITE_GROUP_SETMUL] THEN
+  SIMP_TAC[GROUP_SETMUL_RIGHT_COSET; NORMAL_SUBGROUP_OF_OPPOSITE_GROUP;
            OPPOSITE_GROUP]);;
 
 (* ------------------------------------------------------------------------- *)
@@ -1811,7 +2114,7 @@ let GROUP_SETOP_LEFT_COSET = prove
 let quotient_group = new_definition
  `quotient_group G (n:A->bool) =
         group ({right_coset G n x |x| x IN group_carrier G},
-               n,group_setinv G,group_setop G)`;;
+               n,group_setinv G,group_setmul G)`;;
 
 let QUOTIENT_GROUP = prove
  (`(!G n:A->bool.
@@ -1826,7 +2129,7 @@ let QUOTIENT_GROUP = prove
         ==> group_inv(quotient_group G n) = group_setinv G) /\
    (!G n:A->bool.
         n normal_subgroup_of G
-        ==> group_op(quotient_group G n) = group_setop G)`,
+        ==> group_mul(quotient_group G n) = group_setmul G)`,
   REWRITE_TAC[AND_FORALL_THM; TAUT
    `(p ==> q) /\ (p ==> r) <=> p ==> q /\ r`] THEN
   REPEAT GEN_TAC THEN DISCH_TAC THEN
@@ -1834,24 +2137,24 @@ let QUOTIENT_GROUP = prove
    (ISPEC(rand(rand(snd(strip_forall(concl quotient_group)))))
    (CONJUNCT2 group_tybij)))) THEN
   REWRITE_TAC[GSYM quotient_group] THEN ANTS_TAC THENL
-   [ALL_TAC; SIMP_TAC[group_carrier; group_id; group_inv; group_op]] THEN
+   [ALL_TAC; SIMP_TAC[group_carrier; group_id; group_inv; group_mul]] THEN
   REWRITE_TAC[RIGHT_FORALL_IMP_THM; IMP_CONJ; FORALL_IN_GSPEC] THEN
-  ASM_SIMP_TAC[GROUP_SETOP_RIGHT_COSET; GROUP_SETINV_RIGHT_COSET;
-               GROUP_OP; GROUP_INV] THEN
+  ASM_SIMP_TAC[GROUP_SETMUL_RIGHT_COSET; GROUP_SETINV_RIGHT_COSET;
+               GROUP_MUL; GROUP_INV] THEN
   FIRST_ASSUM(STRIP_ASSUME_TAC o REWRITE_RULE[normal_subgroup_of]) THEN
   FIRST_ASSUM(ASSUME_TAC o MATCH_MP SUBGROUP_OF_IMP_SUBSET) THEN
   REWRITE_TAC[IN_ELIM_THM] THEN REPEAT CONJ_TAC THENL
    [ASM_MESON_TAC[RIGHT_COSET_ID; GROUP_ID];
     ASM_MESON_TAC[GROUP_INV];
-    ASM_MESON_TAC[GROUP_OP];
-    ASM_SIMP_TAC[GROUP_OP_ASSOC];
+    ASM_MESON_TAC[GROUP_MUL];
+    ASM_SIMP_TAC[GROUP_MUL_ASSOC];
     X_GEN_TAC `x:A` THEN DISCH_TAC THEN CONJ_TAC THENL
-     [ASM_SIMP_TAC[right_coset; GROUP_SETOP_ASSOC; SING_SUBSET];
+     [ASM_SIMP_TAC[right_coset; GROUP_SETMUL_ASSOC; SING_SUBSET];
       FIRST_X_ASSUM(MP_TAC o SPEC `x:A`) THEN
       ASM_REWRITE_TAC[] THEN DISCH_THEN(SUBST1_TAC o SYM) THEN
-      ASM_SIMP_TAC[left_coset; GSYM GROUP_SETOP_ASSOC; SING_SUBSET]] THEN
-    ASM_SIMP_TAC[GROUP_SETOP_SUBGROUP];
-    ASM_SIMP_TAC[GROUP_OP_LINV; GROUP_OP_RINV; RIGHT_COSET_ID]]);;
+      ASM_SIMP_TAC[left_coset; GSYM GROUP_SETMUL_ASSOC; SING_SUBSET]] THEN
+    ASM_SIMP_TAC[GROUP_SETMUL_SUBGROUP];
+    ASM_SIMP_TAC[GROUP_MUL_LINV; GROUP_MUL_RINV; RIGHT_COSET_ID]]);;
 
 let QUOTIENT_GROUP_ID = prove
  (`!G n:A->bool.
@@ -1866,19 +2169,45 @@ let QUOTIENT_GROUP_INV = prove
             right_coset G n (group_inv G a)`,
   SIMP_TAC[QUOTIENT_GROUP; GROUP_SETINV_RIGHT_COSET]);;
 
-let QUOTIENT_GROUP_OP = prove
+let QUOTIENT_GROUP_MUL = prove
  (`!G n a b:A.
         n normal_subgroup_of G /\ a IN group_carrier G /\ b IN group_carrier G
-        ==> group_op (quotient_group G n)
+        ==> group_mul (quotient_group G n)
                       (right_coset G n a) (right_coset G n b) =
-            right_coset G n (group_op G a b)`,
-  SIMP_TAC[QUOTIENT_GROUP; GROUP_SETOP_RIGHT_COSET]);;
+            right_coset G n (group_mul G a b)`,
+  SIMP_TAC[QUOTIENT_GROUP; GROUP_SETMUL_RIGHT_COSET]);;
+
+let QUOTIENT_GROUP_DIV = prove
+ (`!G n a b:A.
+        n normal_subgroup_of G /\ a IN group_carrier G /\ b IN group_carrier G
+        ==> group_div (quotient_group G n)
+                      (right_coset G n a) (right_coset G n b) =
+            right_coset G n (group_div G a b)`,
+  SIMP_TAC[group_div; QUOTIENT_GROUP_INV; QUOTIENT_GROUP_MUL; GROUP_INV]);;
+
+let QUOTIENT_GROUP_POW = prove
+ (`!G n (a:A) k.
+        n normal_subgroup_of G /\ a IN group_carrier G
+        ==> group_pow (quotient_group G n) (right_coset G n a) k =
+            right_coset G n (group_pow G a k)`,
+  REWRITE_TAC[RIGHT_FORALL_IMP_THM] THEN REPEAT GEN_TAC THEN STRIP_TAC THEN
+  INDUCT_TAC THEN ASM_SIMP_TAC[group_pow; QUOTIENT_GROUP_MUL; GROUP_POW] THEN
+  ASM_SIMP_TAC[QUOTIENT_GROUP_ID; NORMAL_SUBGROUP_IMP_SUBGROUP;
+               SUBGROUP_OF_IMP_SUBSET; RIGHT_COSET_ID]);;
+
+let QUOTIENT_GROUP_ZPOW = prove
+ (`!G n (a:A) k.
+        n normal_subgroup_of G /\ a IN group_carrier G
+        ==> group_zpow (quotient_group G n) (right_coset G n a) k =
+            right_coset G n (group_zpow G a k)`,
+  REPEAT STRIP_TAC THEN REWRITE_TAC[group_zpow] THEN COND_CASES_TAC THEN
+  ASM_MESON_TAC[QUOTIENT_GROUP_INV; QUOTIENT_GROUP_POW; GROUP_POW]);;
 
 let GROUP_HOMOMORPHISM_RIGHT_COSET = prove
  (`!G n:A->bool.
         n normal_subgroup_of G
         ==> group_homomorphism (G,quotient_group G n) (right_coset G n)`,
-  SIMP_TAC[group_homomorphism; QUOTIENT_GROUP_INV; QUOTIENT_GROUP_OP] THEN
+  SIMP_TAC[group_homomorphism; QUOTIENT_GROUP_INV; QUOTIENT_GROUP_MUL] THEN
   SIMP_TAC[SUBSET; FORALL_IN_IMAGE; QUOTIENT_GROUP] THEN
   SIMP_TAC[normal_subgroup_of; subgroup_of; RIGHT_COSET_ID] THEN SET_TAC[]);;
 
@@ -1939,7 +2268,7 @@ let GROUP_MONOMORPHISM = prove
     ASM_SIMP_TAC[GROUP_ID];
     MAP_EVERY X_GEN_TAC [`x:A`; `y:A`] THEN STRIP_TAC THEN
     FIRST_X_ASSUM(MP_TAC o SPEC `group_div G x y:A`) THEN
-    ASM_SIMP_TAC[group_div; GROUP_OP; GROUP_INV] THEN
+    ASM_SIMP_TAC[group_div; GROUP_MUL; GROUP_INV] THEN
     REWRITE_TAC[GSYM group_div] THEN
     W(MP_TAC o PART_MATCH (lhand o rand) GROUP_DIV_EQ_ID o
       rand o lhand o snd) THEN
@@ -1986,7 +2315,7 @@ let GROUP_ISOMORPHISM_ALT = prove
       group_isomorphism (G,G') f <=>
       IMAGE f (group_carrier G) = group_carrier G' /\
       (!x y. x IN group_carrier G /\ y IN group_carrier G
-             ==> f(group_op G x y) = group_op G' (f x) (f y)) /\
+             ==> f(group_mul G x y) = group_mul G' (f x) (f y)) /\
       (!x. x IN group_carrier G /\ f x = group_id G' ==> x = group_id G)`,
   REPEAT GEN_TAC THEN ASM_CASES_TAC `group_homomorphism (G,G') (f:A->B)` THENL
    [ALL_TAC;
@@ -2000,7 +2329,7 @@ let SUBGROUP_GROUP_KERNEL = prove
  (`!G G' (f:A->B).
         group_homomorphism(G,G') f ==> (group_kernel (G,G') f) subgroup_of G`,
   SIMP_TAC[group_homomorphism; subgroup_of; group_kernel; IN_ELIM_THM; SUBSET;
-           FORALL_IN_IMAGE; GROUP_OP_LID; GROUP_ID; GROUP_OP;
+           FORALL_IN_IMAGE; GROUP_MUL_LID; GROUP_ID; GROUP_MUL;
            GROUP_INV_ID; GROUP_INV]);;
 
 let SUBGROUP_GROUP_IMAGE = prove
@@ -2008,7 +2337,7 @@ let SUBGROUP_GROUP_IMAGE = prove
         group_homomorphism(G,G') f ==> (group_image (G,G') f) subgroup_of G'`,
   SIMP_TAC[group_homomorphism; subgroup_of; group_image; SUBSET;
            FORALL_IN_IMAGE; FORALL_IN_IMAGE_2; IN_IMAGE] THEN
-  MESON_TAC[GROUP_OP; GROUP_INV; GROUP_ID]);;
+  MESON_TAC[GROUP_MUL; GROUP_INV; GROUP_ID]);;
 
 let GROUP_KERNEL_TO_SUBGROUP_GENERATED = prove
  (`!G H s (f:A->B).
@@ -2053,13 +2382,13 @@ let NORMAL_SUBGROUP_GROUP_KERNEL = prove
         group_homomorphism(G,G') f
         ==> (group_kernel (G,G') f) normal_subgroup_of G`,
   SIMP_TAC[NORMAL_SUBGROUP_CONJUGATE; SUBGROUP_GROUP_KERNEL] THEN
-  REWRITE_TAC[group_homomorphism; group_setop] THEN REPEAT STRIP_TAC THEN
+  REWRITE_TAC[group_homomorphism; group_setmul] THEN REPEAT STRIP_TAC THEN
   REWRITE_TAC[SIMPLE_IMAGE; GSYM IMAGE_o; o_DEF;
       SET_RULE `{f x y | P x /\ y IN {a}} = {f x a | P x}`;
       SET_RULE `{f x y | x IN {a} /\ P y} = {f a y | P y}`] THEN
   REWRITE_TAC[SUBSET; FORALL_IN_IMAGE; group_kernel; IN_ELIM_THM] THEN
   RULE_ASSUM_TAC(REWRITE_RULE[SUBSET; FORALL_IN_IMAGE]) THEN
-  ASM_SIMP_TAC[GROUP_INV; GROUP_OP; GROUP_OP_LID; GROUP_OP_LINV]);;
+  ASM_SIMP_TAC[GROUP_INV; GROUP_MUL; GROUP_MUL_LID; GROUP_MUL_LINV]);;
 
 let GROUP_KERNEL_RIGHT_COSET = prove
  (`!G n:A->bool.
@@ -2085,8 +2414,8 @@ let QUOTIENT_GROUP_UNIVERSAL = prove
   MATCH_MP_TAC MONO_EXISTS THEN X_GEN_TAC `g:(A->bool)->B` THEN
   DISCH_TAC THEN ASM_SIMP_TAC[QUOTIENT_GROUP] THEN
   REWRITE_TAC[IMP_CONJ; RIGHT_FORALL_IMP_THM; FORALL_IN_GSPEC] THEN
-  ASM_SIMP_TAC[GROUP_SETINV_RIGHT_COSET; GROUP_SETOP_RIGHT_COSET] THEN
-  ASM_SIMP_TAC[GROUP_OP; GROUP_INV] THEN
+  ASM_SIMP_TAC[GROUP_SETINV_RIGHT_COSET; GROUP_SETMUL_RIGHT_COSET] THEN
+  ASM_SIMP_TAC[GROUP_MUL; GROUP_INV] THEN
   SUBGOAL_THEN `n = right_coset G n (group_id G:A)` SUBST1_TAC THENL
    [ASM_MESON_TAC[RIGHT_COSET_ID; normal_subgroup_of;
                   SUBGROUP_OF_IMP_SUBSET];
@@ -2145,3 +2474,564 @@ let FIRST_GROUP_ISOMORPHISM_THEOREM = prove
    (REWRITE_RULE[group_homomorphism; SUBSET; FORALL_IN_IMAGE]) THEN
   ASM_SIMP_TAC[group_div; GROUP_INV] THEN
   ASM_SIMP_TAC[GSYM group_div; GROUP_DIV_EQ_ID]);;
+
+(* ------------------------------------------------------------------------- *)
+(* Trivial homomorphisms.                                                    *)
+(* ------------------------------------------------------------------------- *)
+
+let trivial_homomorphism = new_definition
+ `trivial_homomorphism(G,G') (f:A->B) <=>
+        group_homomorphism(G,G') f /\
+        !x. x IN group_carrier G ==> f x = group_id G'`;;
+
+let GROUP_KERNEL_IMAGE_TRIVIAL = prove
+ (`!(f:A->B) G G'.
+        group_homomorphism (G,G') f
+        ==> (group_kernel(G,G') f = group_carrier G <=>
+             group_image(G,G') f = {group_id G'})`,
+  REPEAT GEN_TAC THEN
+  REWRITE_TAC[group_homomorphism; group_image; group_kernel] THEN
+  MP_TAC(ISPEC `G:A group` GROUP_ID) THEN SET_TAC[]);;
+
+let TRIVIAL_HOMOMORPHISM_GROUP_KERNEL = prove
+ (`!(f:A->B) G G'.
+        trivial_homomorphism(G,G') f <=>
+        group_homomorphism(G,G') f /\
+        group_kernel(G,G') f = group_carrier G`,
+  REPEAT GEN_TAC THEN
+  REWRITE_TAC[trivial_homomorphism; group_kernel; group_homomorphism] THEN
+  SET_TAC[]);;
+
+let TRIVIAL_HOMOMORPHISM_GROUP_IMAGE = prove
+ (`!(f:A->B) G G'.
+        trivial_homomorphism(G,G') f <=>
+        group_homomorphism(G,G') f /\
+        group_image(G,G') f = {group_id G'}`,
+  MESON_TAC[TRIVIAL_HOMOMORPHISM_GROUP_KERNEL; GROUP_KERNEL_IMAGE_TRIVIAL]);;
+
+let GROUP_HOMOMORPHISM_TRIVIAL = prove
+ (`!G H. group_homomorphism (G,H) (\x. group_id H)`,
+  SIMP_TAC[group_homomorphism; SUBSET; FORALL_IN_IMAGE; GROUP_MUL_LID;
+           GROUP_INV_ID; GROUP_ID]);;
+
+let TRIVIAL_HOMOMORPHISM_TRIVIAL = prove
+ (`!G H. trivial_homomorphism (G,H) (\x. group_id H)`,
+  REWRITE_TAC[trivial_homomorphism; GROUP_HOMOMORPHISM_TRIVIAL]);;
+
+let GROUP_MONOMORPHISM_TRIVIAL = prove
+ (`!G H. group_monomorphism (G,H) (\x. group_id H) <=> trivial_group G`,
+  REWRITE_TAC[group_monomorphism; GROUP_HOMOMORPHISM_TRIVIAL] THEN
+  REWRITE_TAC[TRIVIAL_GROUP_ALT] THEN SET_TAC[]);;
+
+let GROUP_EPIMORPHISM_TRIVIAL = prove
+ (`!G H. group_epimorphism (G,H) (\x. group_id H) <=> trivial_group H`,
+  REWRITE_TAC[group_epimorphism; GROUP_HOMOMORPHISM_TRIVIAL] THEN
+  SIMP_TAC[GROUP_CARRIER_NONEMPTY; SET_RULE
+   `~(s = {}) ==> IMAGE (\x. a) s = {a}`] THEN
+  REWRITE_TAC[trivial_group; EQ_SYM_EQ]);;
+
+let GROUP_ISOMORPHISM_TRIVIAL = prove
+ (`!G H. group_isomorphism (G,H) (\x. group_id H) <=>
+         trivial_group G /\ trivial_group H`,
+  REWRITE_TAC[GSYM GROUP_MONOMORPHISM_EPIMORPHISM] THEN
+  REWRITE_TAC[GROUP_MONOMORPHISM_TRIVIAL; GROUP_EPIMORPHISM_TRIVIAL]);;
+
+(* ------------------------------------------------------------------------- *)
+(* Abelian groups.                                                           *)
+(* ------------------------------------------------------------------------- *)
+
+let abelian_group = new_definition
+ `abelian_group (G:A group) <=>
+  !x y. x IN group_carrier G /\ y IN group_carrier G
+        ==> group_mul G x y = group_mul G y x`;;
+
+let ABELIAN_GROUP_MUL_AC = prove
+ (`!G:A group.
+        abelian_group G <=>
+        (!x y. x IN group_carrier G /\ y IN group_carrier G
+               ==> group_mul G x y = group_mul G y x) /\
+        (!x y z. x IN group_carrier G /\ y IN group_carrier G /\
+                 z IN group_carrier G
+                 ==> group_mul G (group_mul G x y) z =
+                     group_mul G x (group_mul G y z)) /\
+        (!x y z. x IN group_carrier G /\ y IN group_carrier G /\
+                 z IN group_carrier G
+                 ==> group_mul G x (group_mul G y z) =
+                     group_mul G y (group_mul G x z))`,
+  REWRITE_TAC[abelian_group] THEN MESON_TAC[GROUP_MUL_ASSOC]);;
+
+let GROUP_SETMUL_SYM = prove
+ (`!G g h:A->bool.
+        abelian_group G /\ g SUBSET group_carrier G /\ h SUBSET group_carrier G
+        ==> group_setmul G g h = group_setmul G h g`,
+  REWRITE_TAC[abelian_group; group_setmul] THEN SET_TAC[]);;
+
+let SUBGROUP_SETMUL = prove
+ (`!G g h:A->bool.
+        abelian_group G /\ g subgroup_of G /\ h subgroup_of G
+        ==> (group_setmul G g h) subgroup_of G`,
+  MESON_TAC[GROUP_SETMUL_SYM; SUBGROUP_SETMUL_EQ; subgroup_of]);;
+
+let ABELIAN_OPPOSITE_GROUP = prove
+ (`!G:A group. abelian_group (opposite_group G) <=> abelian_group G`,
+  SIMP_TAC[abelian_group; OPPOSITE_GROUP_MUL; OPPOSITE_GROUP] THEN
+  MESON_TAC[]);;
+
+let ABELIAN_GROUP_NORMAL_SUBGROUP = prove
+ (`!G n:A->bool.
+        abelian_group G ==> (n normal_subgroup_of G <=> n subgroup_of G)`,
+  REWRITE_TAC[normal_subgroup_of; left_coset; right_coset; subgroup_of] THEN
+  MESON_TAC[GROUP_SETMUL_SYM; SING_SUBSET]);;
+
+let ABELIAN_GROUP_QUOTIENT_GROUP = prove
+ (`!G n:A->bool.
+     abelian_group G /\ n subgroup_of G ==> abelian_group(quotient_group G n)`,
+  REPEAT STRIP_TAC THEN
+  ASM_SIMP_TAC[abelian_group; QUOTIENT_GROUP; ABELIAN_GROUP_NORMAL_SUBGROUP;
+               IMP_CONJ; RIGHT_FORALL_IMP_THM; FORALL_IN_GSPEC] THEN
+  ASM_SIMP_TAC[GROUP_SETMUL_SYM; RIGHT_COSET; SUBGROUP_OF_IMP_SUBSET]);;
+
+let ABELIAN_SUBGROUP_GENERATED = prove
+ (`!G h:A->bool.
+        abelian_group G ==> abelian_group(subgroup_generated G h)`,
+  SIMP_TAC[abelian_group; SUBGROUP_GENERATED] THEN
+  REWRITE_TAC[IN_INTERS; IN_ELIM_THM] THEN REPEAT STRIP_TAC THEN
+  REPEAT(FIRST_X_ASSUM(MP_TAC o SPEC `group_carrier(G:A group)`)) THEN
+  ASM_REWRITE_TAC[CARRIER_SUBGROUP_OF; INTER_SUBSET] THEN
+  ASM_MESON_TAC[]);;
+
+let TRIVIAL_IMP_ABELIAN_GROUP = prove
+ (`!G:A group. trivial_group G ==> abelian_group G`,
+  SIMP_TAC[trivial_group; abelian_group; IN_SING]);;
+
+let ABELIAN_SINGLETON_GROUP = prove
+ (`!a:A. abelian_group(singleton_group a)`,
+  SIMP_TAC[TRIVIAL_IMP_ABELIAN_GROUP; TRIVIAL_GROUP_SINGLETON_GROUP]);;
+
+let ABELIAN_GROUP_HOMOMORPHISM_GROUP_MUL = prove
+ (`!(f:A->B) g A B.
+        abelian_group B /\
+        group_homomorphism(A,B) f /\ group_homomorphism(A,B) g
+        ==> group_homomorphism(A,B) (\x. group_mul B (f x) (g x))`,
+  REWRITE_TAC[group_homomorphism; ABELIAN_GROUP_MUL_AC] THEN
+  REWRITE_TAC[SUBSET; FORALL_IN_IMAGE] THEN
+  SIMP_TAC[GROUP_MUL_LID; GROUP_ID; GROUP_MUL; GROUP_INV_MUL; GROUP_INV]);;
+
+let ABELIAN_GROUP_EPIMORPHIC_IMAGE = prove
+ (`!G H (f:A->B).
+     group_epimorphism(G,H) f /\ abelian_group G ==> abelian_group H`,
+  REPEAT GEN_TAC THEN
+  SIMP_TAC[group_epimorphism; group_homomorphism; abelian_group] THEN
+  DISCH_THEN(STRIP_ASSUME_TAC o GSYM) THEN
+  ASM_REWRITE_TAC[FORALL_IN_IMAGE_2] THEN ASM SET_TAC[]);;
+
+let ISOMORPHIC_GROUP_ABELIANNESS = prove
+ (`!(G:A group) (H:B group).
+        G isomorphic_group H ==> (abelian_group G <=> abelian_group H)`,
+  REPEAT STRIP_TAC THEN EQ_TAC THEN
+  MATCH_MP_TAC(REWRITE_RULE[IMP_CONJ] ABELIAN_GROUP_EPIMORPHIC_IMAGE) THEN
+  ASM_MESON_TAC[isomorphic_group; ISOMORPHIC_GROUP_SYM;
+                GROUP_MONOMORPHISM_EPIMORPHISM]);;
+
+(* ------------------------------------------------------------------------- *)
+(* Cyclic groups.                                                            *)
+(* ------------------------------------------------------------------------- *)
+
+let SUBGROUP_OF_POWERS = prove
+ (`!G (x:A).
+      x IN group_carrier G ==> {group_zpow G x n | n IN (:int)} subgroup_of G`,
+  REWRITE_TAC[subgroup_of; IMP_CONJ; RIGHT_FORALL_IMP_THM] THEN
+  REWRITE_TAC[SUBSET; FORALL_IN_GSPEC; IN_UNIV] THEN
+  SIMP_TAC[GROUP_ZPOW; GSYM GROUP_ZPOW_ADD; GSYM GROUP_ZPOW_NEG] THEN
+  REWRITE_TAC[IN_ELIM_THM] THEN MESON_TAC[GROUP_NPOW; group_pow]);;
+
+let CARRIER_SUBGROUP_GENERATED_BY_SING = prove
+ (`!G x:A.
+        x IN group_carrier G
+        ==> group_carrier(subgroup_generated G {x}) =
+            {group_zpow G x n | n IN (:int)}`,
+  REPEAT STRIP_TAC THEN MATCH_MP_TAC SUBSET_ANTISYM THEN CONJ_TAC THENL
+   [MATCH_MP_TAC SUBGROUP_GENERATED_MINIMAL THEN
+    ASM_SIMP_TAC[SUBGROUP_OF_POWERS; SING_SUBSET; IN_ELIM_THM] THEN
+    ASM_MESON_TAC[GROUP_ZPOW_1; IN_UNIV];
+    MP_TAC(ISPECL [`G:A group`; `{x:A}`] SUBGROUP_SUBGROUP_GENERATED) THEN
+    REWRITE_TAC[subgroup_of; SUBSET; FORALL_IN_GSPEC; IN_UNIV] THEN
+    STRIP_TAC THEN X_GEN_TAC `n:int` THEN
+    DISJ_CASES_THEN MP_TAC(SPEC `n:int` INT_IMAGE) THEN
+    DISCH_THEN(X_CHOOSE_THEN `m:num` SUBST1_TAC) THEN
+    ASM_SIMP_TAC[GROUP_ZPOW_NEG; GROUP_NPOW] THEN
+    TRY(FIRST_X_ASSUM MATCH_MP_TAC) THEN SPEC_TAC(`m:num`,`m:num`) THEN
+    INDUCT_TAC THEN ASM_SIMP_TAC[group_pow] THEN
+    FIRST_X_ASSUM MATCH_MP_TAC THEN ASM_REWRITE_TAC[] THEN
+    REWRITE_TAC[GSYM SING_SUBSET] THEN
+    MATCH_MP_TAC SUBGROUP_GENERATED_SUBSET_CARRIER_SUBSET THEN
+    ASM_REWRITE_TAC[SING_SUBSET]]);;
+
+let cyclic_group = new_definition
+ `cyclic_group G <=>
+        ?x. x IN group_carrier G /\ subgroup_generated G {x} = G`;;
+
+let CYCLIC_GROUP = prove
+ (`!G:A group.
+        cyclic_group G <=>
+        ?x. x IN group_carrier G /\
+            group_carrier G = {group_zpow G x n | n IN (:int)}`,
+  GEN_TAC THEN REWRITE_TAC[cyclic_group] THEN MATCH_MP_TAC(MESON[]
+   `(!x. P x ==> (Q x <=> R x))
+    ==> ((?x. P x /\ Q x) <=> (?x. P x /\ R x))`) THEN
+  SIMP_TAC[GSYM CARRIER_SUBGROUP_GENERATED_BY_SING] THEN REPEAT STRIP_TAC THEN
+  REWRITE_TAC[GROUPS_EQ; CONJUNCT2 SUBGROUP_GENERATED] THEN MESON_TAC[]);;
+
+let CYCLIC_IMP_ABELIAN_GROUP = prove
+ (`!G:A group. cyclic_group G ==> abelian_group G`,
+  SIMP_TAC[CYCLIC_GROUP; abelian_group; LEFT_IMP_EXISTS_THM] THEN
+  REWRITE_TAC[IMP_CONJ; RIGHT_FORALL_IMP_THM; FORALL_IN_GSPEC] THEN
+  SIMP_TAC[GSYM GROUP_ZPOW_ADD] THEN REWRITE_TAC[INT_ADD_SYM]);;
+
+let TRIVIAL_IMP_CYCLIC_GROUP = prove
+ (`!G:A group. trivial_group G ==> cyclic_group G`,
+  REWRITE_TAC[trivial_group; cyclic_group] THEN
+  REPEAT STRIP_TAC THEN EXISTS_TAC `group_id G:A` THEN
+  ASM_MESON_TAC[SUBGROUP_GENERATED_GROUP_CARRIER; GROUP_ID]);;
+
+let CYCLIC_GROUP_EPIMORPHIC_IMAGE = prove
+ (`!G H (f:A->B).
+        group_epimorphism(G,H) f /\ cyclic_group G ==> cyclic_group H`,
+  REPEAT GEN_TAC THEN REWRITE_TAC[group_epimorphism] THEN
+  DISCH_THEN(CONJUNCTS_THEN2 (STRIP_ASSUME_TAC o GSYM) MP_TAC) THEN
+  REWRITE_TAC[CYCLIC_GROUP] THEN
+  DISCH_THEN(X_CHOOSE_THEN `x:A` STRIP_ASSUME_TAC) THEN
+  EXISTS_TAC `(f:A->B) x` THEN
+  FIRST_ASSUM(ASSUME_TAC o MATCH_MP (SET_RULE
+   `t = IMAGE f s ==> !x. x IN s ==> f x IN t`)) THEN
+  FIRST_ASSUM(fun th ->
+    ASM_SIMP_TAC[GSYM(MATCH_MP GROUP_HOMOMORPHISM_ZPOW th)]) THEN
+  SET_TAC[]);;
+
+let ISOMORPHIC_GROUP_CYCLICITY = prove
+ (`!(G:A group) (H:B group).
+        G isomorphic_group H ==> (cyclic_group G <=> cyclic_group H)`,
+  REPEAT STRIP_TAC THEN EQ_TAC THEN
+  MATCH_MP_TAC(REWRITE_RULE[IMP_CONJ] CYCLIC_GROUP_EPIMORPHIC_IMAGE) THEN
+  ASM_MESON_TAC[isomorphic_group; ISOMORPHIC_GROUP_SYM;
+                GROUP_MONOMORPHISM_EPIMORPHISM]);;
+
+let SUBGROUP_OF_CYCLIC_GROUP_EXPLICIT = prove
+ (`!G h x:A.
+        x IN group_carrier G /\ h subgroup_of (subgroup_generated G {x})
+        ==> ?k. h = {group_zpow G x (&k * n) | n IN (:int)}`,
+  REPEAT GEN_TAC THEN REWRITE_TAC[IMP_CONJ] THEN
+  ASM_CASES_TAC `(h:A->bool) subgroup_of G` THENL
+   [ALL_TAC; ASM_MESON_TAC[SUBGROUP_OF_SUBGROUP_GENERATED_REV]] THEN
+  SIMP_TAC[subgroup_of; CARRIER_SUBGROUP_GENERATED_BY_SING] THEN
+  REWRITE_TAC[SUBGROUP_GENERATED] THEN REPEAT STRIP_TAC THEN
+  ASM_CASES_TAC `h SUBSET {group_zpow G (x:A) (&0)}` THENL
+   [EXISTS_TAC `0` THEN
+    ASM_REWRITE_TAC[INT_MUL_LZERO; GSYM SUBSET_ANTISYM_EQ;
+                    SET_RULE `{a |x| x IN UNIV} = {a}`] THEN
+    ASM_REWRITE_TAC[GROUP_ZPOW_0; SING_SUBSET];
+    ALL_TAC] THEN
+  SUBGOAL_THEN `?n. 0 < n /\ group_pow G (x:A) n IN h` MP_TAC THENL
+   [FIRST_ASSUM(MP_TAC o MATCH_MP (SET_RULE
+     `h SUBSET {f x | x IN (:int)} ==> ~(h SUBSET {f(&0)})
+      ==> ?n. ~(n = &0) /\ f n IN h`)) THEN
+    ASM_REWRITE_TAC[] THEN
+    DISCH_THEN(X_CHOOSE_THEN `n:int` STRIP_ASSUME_TAC) THEN
+    EXISTS_TAC `num_of_int(abs n)` THEN
+    REWRITE_TAC[GSYM GROUP_NPOW; GSYM INT_OF_NUM_LT] THEN
+    SIMP_TAC[INT_OF_NUM_OF_INT; INT_ABS_POS] THEN
+    ASM_REWRITE_TAC[GSYM INT_ABS_NZ] THEN REWRITE_TAC[INT_ABS] THEN
+    COND_CASES_TAC THEN ASM_SIMP_TAC[GROUP_ZPOW_NEG];
+    GEN_REWRITE_TAC LAND_CONV [num_WOP]] THEN
+  MATCH_MP_TAC MONO_EXISTS THEN X_GEN_TAC `k:num` THEN
+  REWRITE_TAC[TAUT `(p ==> ~(q /\ r)) <=> q /\ p ==> ~r`] THEN
+  STRIP_TAC THEN MATCH_MP_TAC SUBSET_ANTISYM THEN
+  REWRITE_TAC[SUBSET; FORALL_IN_GSPEC] THEN
+  REWRITE_TAC[IN_ELIM_THM; IN_UNIV] THEN
+  MATCH_MP_TAC(TAUT `q /\ (q ==> p) ==> p /\ q`) THEN CONJ_TAC THENL
+   [MP_TAC(ISPECL [`subgroup_generated G (h:A->bool)`; `group_pow G x k:A`]
+        GROUP_ZPOW) THEN
+    REWRITE_TAC[GROUP_ZPOW_SUBGROUP_GENERATED] THEN
+    ASM_SIMP_TAC[CARRIER_SUBGROUP_GENERATED_SUBGROUP] THEN
+    ASM_SIMP_TAC[GROUP_ZPOW_MUL; GROUP_NPOW];
+    DISCH_THEN(LABEL_TAC "*")] THEN
+  FIRST_X_ASSUM(MATCH_MP_TAC o MATCH_MP (SET_RULE
+   `h SUBSET {f x | x IN s} ==> (!x. f x IN h ==> P(f x))
+   ==> !y. y IN h ==> P y`)) THEN
+  X_GEN_TAC `m:int` THEN DISCH_THEN(fun th ->
+    EXISTS_TAC `m div (&k)` THEN MP_TAC th) THEN
+  ONCE_REWRITE_TAC[INT_MUL_SYM] THEN
+  MP_TAC(SPECL [`m:int`; `&k:int`] INT_DIVISION) THEN
+  ASM_REWRITE_TAC[INT_OF_NUM_EQ; GSYM LT_NZ; INT_ABS_NUM] THEN
+  SPEC_TAC(`m div &k`,`q:int`) THEN
+  SPEC_TAC(`m rem &k`,`r:int`) THEN ONCE_REWRITE_TAC[TAUT
+   `p /\ q /\ r ==> s <=> q ==> r /\ p ==> s`] THEN
+  REWRITE_TAC[GSYM INT_FORALL_POS; RIGHT_FORALL_IMP_THM] THEN
+  MAP_EVERY X_GEN_TAC [`m:num`; `q:int`] THEN
+  REWRITE_TAC[INT_OF_NUM_LT] THEN
+  DISCH_THEN(CONJUNCTS_THEN2 ASSUME_TAC SUBST1_TAC) THEN
+  ASM_CASES_TAC `m = 0` THEN ASM_REWRITE_TAC[INT_ADD_RID] THEN
+  DISCH_TAC THEN
+  FIRST_X_ASSUM(MP_TAC o SPEC `m:num`) THEN ASM_REWRITE_TAC[LT_NZ] THEN
+  MATCH_MP_TAC(TAUT `p ==> ~p ==> q`) THEN REWRITE_TAC[GSYM GROUP_NPOW] THEN
+  SUBST1_TAC(INT_ARITH `&m:int = --(&k * q) + (q * &k + &m)`) THEN
+  W(MP_TAC o PART_MATCH (lhand o rand) GROUP_ZPOW_ADD o lhand o snd) THEN
+  ASM_REWRITE_TAC[] THEN DISCH_THEN(SUBST1_TAC) THEN
+  FIRST_X_ASSUM MATCH_MP_TAC THEN ASM_REWRITE_TAC[] THEN
+  ASM_SIMP_TAC[GROUP_ZPOW_NEG]);;
+
+let SUBGROUP_OF_CYCLIC_GROUP = prove
+ (`!G h:A->bool.
+        cyclic_group G /\ h subgroup_of G
+        ==> cyclic_group(subgroup_generated G h)`,
+  REPEAT STRIP_TAC THEN REWRITE_TAC[CYCLIC_GROUP] THEN
+  ASM_SIMP_TAC[CARRIER_SUBGROUP_GENERATED_SUBGROUP] THEN
+  FIRST_ASSUM(MP_TAC o GEN_REWRITE_RULE I [cyclic_group]) THEN
+  DISCH_THEN(X_CHOOSE_THEN `x:A` STRIP_ASSUME_TAC) THEN
+  MP_TAC(ISPECL [`G:A group`; `h:A->bool`; `x:A`]
+   SUBGROUP_OF_CYCLIC_GROUP_EXPLICIT) THEN
+  ASM_REWRITE_TAC[GROUP_ZPOW_SUBGROUP_GENERATED] THEN
+  ASM_SIMP_TAC[GROUP_ZPOW_MUL] THEN
+  DISCH_THEN(X_CHOOSE_TAC `k:num`) THEN
+  EXISTS_TAC `group_zpow G x (&k):A` THEN
+  ASM_REWRITE_TAC[IN_ELIM_THM] THEN EXISTS_TAC `&1:int` THEN
+  ASM_SIMP_TAC[IN_UNIV; GROUP_ZPOW_1; GROUP_ZPOW]);;
+
+let CYCLIC_GROUP_QUOTIENT_GROUP = prove
+ (`!G n:A->bool.
+     cyclic_group G /\ n subgroup_of G ==> cyclic_group(quotient_group G n)`,
+  REPEAT GEN_TAC THEN
+  ASM_CASES_TAC `(n:A->bool) normal_subgroup_of G` THENL
+   [ALL_TAC;
+    ASM_MESON_TAC[ABELIAN_GROUP_NORMAL_SUBGROUP;
+                  CYCLIC_IMP_ABELIAN_GROUP]] THEN
+  REWRITE_TAC[CYCLIC_GROUP] THEN DISCH_THEN(CONJUNCTS_THEN2
+   (X_CHOOSE_THEN `x:A` STRIP_ASSUME_TAC) ASSUME_TAC) THEN
+  EXISTS_TAC `right_coset G n (x:A)` THEN
+  ASM_SIMP_TAC[QUOTIENT_GROUP] THEN
+  REWRITE_TAC[SIMPLE_IMAGE; GSYM IMAGE_o; ETA_AX] THEN CONJ_TAC THENL
+   [REWRITE_TAC[IN_IMAGE; IN_UNIV; o_THM] THEN EXISTS_TAC `&1:int` THEN
+    ASM_SIMP_TAC[GROUP_ZPOW_1];
+    MATCH_MP_TAC(SET_RULE
+     `(!x. x IN s ==> f x = g x) ==> IMAGE f s = IMAGE g s`) THEN
+    ASM_SIMP_TAC[QUOTIENT_GROUP_ZPOW; o_THM]]);;
+
+let NO_PROPER_SUBGROUPS_IMP_CYCLIC = prove
+ (`!G:A group.
+        (!h. h subgroup_of G ==> h SUBSET {group_id G} \/ h = group_carrier G)
+        ==> cyclic_group G`,
+  REPEAT STRIP_TAC THEN ASM_CASES_TAC `trivial_group(G:A group)` THEN
+  ASM_SIMP_TAC[TRIVIAL_IMP_CYCLIC_GROUP] THEN FIRST_X_ASSUM
+   (MP_TAC o GEN_REWRITE_RULE RAND_CONV [TRIVIAL_GROUP_SUBSET]) THEN
+  REWRITE_TAC[SET_RULE `~(s SUBSET {a}) <=> ?x. x IN s /\ ~(x = a)`] THEN
+  REWRITE_TAC[cyclic_group] THEN
+  MATCH_MP_TAC MONO_EXISTS THEN X_GEN_TAC `a:A` THEN STRIP_TAC THEN
+  ASM_REWRITE_TAC[GROUPS_EQ; CONJUNCT2 SUBGROUP_GENERATED] THEN
+  FIRST_X_ASSUM(MP_TAC o SPEC
+   `group_carrier (subgroup_generated G {a:A})`) THEN
+  REWRITE_TAC[SUBGROUP_SUBGROUP_GENERATED] THEN
+  MATCH_MP_TAC(TAUT `~p ==> p \/ q ==> q`) THEN
+  REWRITE_TAC[SUBSET] THEN DISCH_THEN(MP_TAC o SPEC `a:A`) THEN
+  ASM_SIMP_TAC[IN_SING; SUBGROUP_GENERATED_INC; IN_SING; SING_SUBSET]);;
+
+let [FINITE_CYCLIC_SUBGROUP; INFINITE_CYCLIC_SUBGROUP;
+     FINITE_CYCLIC_SUBGROUP_ALT; INFINITE_CYCLIC_SUBGROUP_ALT] =
+ (CONJUNCTS o prove)
+ (`(!G x:A.
+        x IN group_carrier G
+        ==> (FINITE(group_carrier(subgroup_generated G {x})) <=>
+             ?n. ~(n = 0) /\ group_pow G x n = group_id G)) /\
+   (!G x:A.
+        x IN group_carrier G
+        ==> (INFINITE(group_carrier(subgroup_generated G {x})) <=>
+             !m n. group_pow G x m = group_pow G x n ==> m = n)) /\
+   (!G x:A.
+        x IN group_carrier G
+        ==> (FINITE(group_carrier(subgroup_generated G {x})) <=>
+             ?n. ~(n = &0) /\ group_zpow G x n = group_id G)) /\
+   (!G x:A.
+        x IN group_carrier G
+        ==> (INFINITE(group_carrier(subgroup_generated G {x})) <=>
+             !m n. group_zpow G x m = group_zpow G x n ==> m = n))`,
+  REWRITE_TAC[INFINITE; AND_FORALL_THM] THEN REPEAT GEN_TAC THEN
+  ASM_CASES_TAC `(x:A) IN group_carrier G` THEN ASM_REWRITE_TAC[] THEN
+  MATCH_MP_TAC(TAUT
+   `(r ==> ~p) /\ (r' ==> r) /\ (~r' ==> q) /\ (q ==> q') /\ (q' ==> p)
+    ==> (p <=> q) /\ (~p <=> r) /\ (p <=> q') /\ (~p <=> r')`) THEN
+  REPEAT CONJ_TAC THENL
+   [DISCH_THEN(MP_TAC o SPEC `(:num)` o MATCH_MP INFINITE_IMAGE_INJ) THEN
+    ASM_SIMP_TAC[num_INFINITE; CARRIER_SUBGROUP_GENERATED_BY_SING] THEN
+    REWRITE_TAC[INFINITE; CONTRAPOS_THM] THEN
+    MATCH_MP_TAC(REWRITE_RULE[IMP_CONJ_ALT] FINITE_SUBSET) THEN
+    REWRITE_TAC[GSYM GROUP_NPOW] THEN SET_TAC[];
+    REWRITE_TAC[GSYM GROUP_NPOW; GSYM INT_OF_NUM_EQ] THEN SET_TAC[];
+    REWRITE_TAC[NOT_FORALL_THM; LEFT_IMP_EXISTS_THM; NOT_IMP] THEN
+    MATCH_MP_TAC INT_WLOG_LT THEN REWRITE_TAC[] THEN
+    CONJ_TAC THENL [MESON_TAC[]; ALL_TAC] THEN
+    MAP_EVERY X_GEN_TAC [`m:int`; `n:int`] THEN REPEAT STRIP_TAC THEN
+    EXISTS_TAC `num_of_int(n - m)` THEN
+    ASM_SIMP_TAC[GSYM GROUP_NPOW; INT_OF_NUM_OF_INT; INT_LT_IMP_LE;
+                 INT_SUB_LT; GSYM INT_OF_NUM_EQ; INT_SUB_0; GROUP_ZPOW_SUB;
+                 GROUP_DIV_REFL; GROUP_ZPOW];
+    REWRITE_TAC[GSYM INT_OF_NUM_EQ; GSYM GROUP_NPOW] THEN MESON_TAC[];
+    DISCH_TAC THEN
+    SUBGOAL_THEN `?n. ~(n = 0) /\ group_pow G (x:A) n = group_id G`
+    STRIP_ASSUME_TAC THENL
+     [FIRST_X_ASSUM(X_CHOOSE_THEN `n:int` STRIP_ASSUME_TAC) THEN
+      EXISTS_TAC `num_of_int(abs n)` THEN
+      REWRITE_TAC[GSYM GROUP_NPOW; GSYM INT_OF_NUM_EQ] THEN
+      SIMP_TAC[INT_OF_NUM_OF_INT; INT_ABS_POS; INT_ABS_ZERO] THEN
+      ASM_REWRITE_TAC[INT_ABS] THEN COND_CASES_TAC THEN
+      ASM_SIMP_TAC[GROUP_ZPOW_NEG; GROUP_INV_ID];
+      MATCH_MP_TAC FINITE_SUBSET THEN
+      EXISTS_TAC `IMAGE (group_pow G (x:A)) (0..n)` THEN
+      ASM_SIMP_TAC[FINITE_IMAGE; FINITE_NUMSEG] THEN
+      ASM_SIMP_TAC[CARRIER_SUBGROUP_GENERATED_BY_SING; SUBSET] THEN
+      REWRITE_TAC[FORALL_IN_GSPEC; IN_UNIV; IN_IMAGE; IN_NUMSEG; LE_0] THEN
+      X_GEN_TAC `a:int` THEN
+      MP_TAC(ISPECL [`a:int`; `&n:int`] INT_DIVISION) THEN
+      ASM_REWRITE_TAC[INT_OF_NUM_EQ] THEN
+      DISCH_THEN(CONJUNCTS_THEN2 SUBST1_TAC MP_TAC) THEN
+      SPEC_TAC(`a rem &n`,`b:int`) THEN ONCE_REWRITE_TAC[INT_MUL_SYM] THEN
+      REWRITE_TAC[IMP_CONJ; GSYM INT_FORALL_POS; INT_ABS_NUM;
+                  INT_OF_NUM_LT] THEN
+      X_GEN_TAC `m:num` THEN DISCH_TAC THEN EXISTS_TAC `m:num` THEN
+      ASM_SIMP_TAC[LT_IMP_LE; GROUP_ZPOW_ADD; GROUP_ZPOW_MUL] THEN
+      ASM_REWRITE_TAC[GROUP_NPOW; GROUP_ZPOW_ID] THEN
+      ASM_SIMP_TAC[GROUP_MUL_LID; GROUP_POW]]]);;
+
+(* ------------------------------------------------------------------------- *)
+(* The additive group of integers.                                           *)
+(* ------------------------------------------------------------------------- *)
+
+let integer_group = new_definition
+ `integer_group = group((:int),&0,(--),(+))`;;
+
+let INTEGER_GROUP = prove
+ (`group_carrier integer_group = (:int) /\
+   group_id integer_group = &0 /\
+   group_inv integer_group = (--) /\
+   group_mul integer_group = (+)`,
+  MP_TAC(fst(EQ_IMP_RULE
+   (ISPEC(rand(rand(snd(strip_forall(concl integer_group)))))
+   (CONJUNCT2 group_tybij)))) THEN
+  REWRITE_TAC[GSYM integer_group] THEN REWRITE_TAC[IN_UNIV] THEN
+  ANTS_TAC THENL [INT_ARITH_TAC; ALL_TAC] THEN
+  SIMP_TAC[group_carrier; group_id; group_inv; group_mul]);;
+
+let GROUP_ENDOMORPHISM_INTEGER_GROUP_MUL = prove
+ (`!c. group_endomorphism integer_group (\x. c * x)`,
+  REWRITE_TAC[group_endomorphism; group_homomorphism; INTEGER_GROUP] THEN
+  REWRITE_TAC[IN_UNIV; SUBSET_UNIV] THEN INT_ARITH_TAC);;
+
+let GROUP_ENDOMORPHISM_INTEGER_GROUP_EXPLICIT = prove
+ (`!f. group_endomorphism integer_group f ==> f = \x. f(&1) * x`,
+  REWRITE_TAC[group_endomorphism; group_homomorphism; INTEGER_GROUP] THEN
+  REWRITE_TAC[IN_UNIV; SUBSET_UNIV] THEN REPEAT STRIP_TAC THEN
+  GEN_REWRITE_TAC I [FUN_EQ_THM] THEN X_GEN_TAC `x:int` THEN
+  REWRITE_TAC[] THEN MP_TAC(SPEC `x:int` INT_IMAGE) THEN
+  DISCH_THEN(DISJ_CASES_THEN MP_TAC) THEN SIMP_TAC[LEFT_IMP_EXISTS_THM] THEN
+  SPEC_TAC(`x:int`,`x:int`) THEN GEN_REWRITE_TAC I [SWAP_FORALL_THM] THEN
+  ASM_REWRITE_TAC[FORALL_UNWIND_THM2; INT_ARITH
+   `--x:int = y * --z <=> x = y * z`] THEN
+  INDUCT_TAC THEN ASM_REWRITE_TAC[INT_MUL_RZERO] THEN
+  ASM_REWRITE_TAC[GSYM INT_OF_NUM_SUC] THEN INT_ARITH_TAC);;
+
+let GROUP_ENDOMORPHISM_INTEGER_GROUP_EQ,
+    GROUP_ENDOMORPHISM_INTEGER_GROUP_EQ_ALT =
+ (CONJ_PAIR o prove)
+ (`(!f. group_endomorphism integer_group f <=> ?c. f = \x. c * x) /\
+   (!f. group_endomorphism integer_group f <=> ?!c. f = \x. c * x)`,
+  REWRITE_TAC[AND_FORALL_THM] THEN GEN_TAC THEN MATCH_MP_TAC(MESON[]
+   `(!c. P(m c)) /\ (!f. P f ==> ?c. f = m c) /\
+    (!c d. m c = m d ==> c = d)
+    ==> (P f <=> ?c. f = m c) /\ (P f <=> ?!c. f = m c)`) THEN
+  REWRITE_TAC[GROUP_ENDOMORPHISM_INTEGER_GROUP_MUL] THEN CONJ_TAC THENL
+   [X_GEN_TAC `f:int->int` THEN DISCH_TAC THEN
+    EXISTS_TAC `(f:int->int) (&1)` THEN
+   MATCH_MP_TAC GROUP_ENDOMORPHISM_INTEGER_GROUP_EXPLICIT THEN
+   ASM_REWRITE_TAC[];
+   REWRITE_TAC[FUN_EQ_THM] THEN MESON_TAC[INT_MUL_RID]]);;
+
+let GROUP_HOMOMORPHISM_GROUP_ZPOW = prove
+ (`!G x:A. x IN group_carrier G
+           ==> group_homomorphism(integer_group,G) (group_zpow G x)`,
+  REWRITE_TAC[group_homomorphism; INTEGER_GROUP; SUBSET; FORALL_IN_IMAGE] THEN
+  SIMP_TAC[IN_UNIV; GROUP_ZPOW_ADD; GROUP_ZPOW_NEG;
+           GROUP_ZPOW_0; GROUP_ZPOW]);;
+
+let GROUP_EPIMORPHISM_GROUP_ZPOW = prove
+ (`!G x:A. x IN group_carrier G
+           ==> group_epimorphism (integer_group,subgroup_generated G {x})
+                                 (group_zpow G x)`,
+  SIMP_TAC[group_epimorphism; INTEGER_GROUP; SIMPLE_IMAGE; ETA_AX;
+           CARRIER_SUBGROUP_GENERATED_BY_SING] THEN
+  REPEAT STRIP_TAC THEN
+  ONCE_REWRITE_TAC[GSYM SUBGROUP_GENERATED_BY_SUBGROUP_GENERATED] THEN
+  MATCH_MP_TAC GROUP_HOMOMORPHISM_INTO_SUBGROUP THEN
+  ASM_SIMP_TAC[GROUP_HOMOMORPHISM_GROUP_ZPOW] THEN
+  ASM_SIMP_TAC[CARRIER_SUBGROUP_GENERATED_BY_SING; INTEGER_GROUP] THEN
+  SET_TAC[]);;
+
+let GROUP_ISOMORPHISM_GROUP_ZPOW = prove
+ (`!G x:A. INFINITE(group_carrier(subgroup_generated G {x})) /\
+           x IN group_carrier G
+           ==> group_isomorphism (integer_group,subgroup_generated G {x})
+                                 (group_zpow G x)`,
+  REPEAT STRIP_TAC THEN
+  FIRST_ASSUM(MP_TAC o MATCH_MP GROUP_EPIMORPHISM_GROUP_ZPOW) THEN
+  SIMP_TAC[GSYM GROUP_MONOMORPHISM_EPIMORPHISM;
+           group_monomorphism; group_epimorphism] THEN
+  DISCH_THEN(K ALL_TAC) THEN REWRITE_TAC[INTEGER_GROUP; IN_UNIV] THEN
+  ASM_MESON_TAC[INFINITE_CYCLIC_SUBGROUP_ALT]);;
+
+let ISOMORPHIC_GROUP_INFINITE_CYCLIC_INTEGER = prove
+ (`!G:A group.
+        cyclic_group G /\ INFINITE(group_carrier G)
+        ==> G isomorphic_group integer_group`,
+  REPEAT STRIP_TAC THEN ONCE_REWRITE_TAC[ISOMORPHIC_GROUP_SYM] THEN
+  FIRST_X_ASSUM(MP_TAC o GEN_REWRITE_RULE I [cyclic_group]) THEN
+  DISCH_THEN(X_CHOOSE_THEN `x:A` STRIP_ASSUME_TAC) THEN
+  MP_TAC(ISPECL [`G:A group`; `x:A`] GROUP_ISOMORPHISM_GROUP_ZPOW) THEN
+  ASM_REWRITE_TAC[GROUP_ISOMORPHISM_IMP_ISOMORPHIC]);;
+
+let ISOMORPHIC_GROUP_INFINITE_CYCLIC_GROUPS = prove
+ (`!(G:A group) (H:B group).
+        cyclic_group G /\ INFINITE(group_carrier G) /\
+        cyclic_group H /\ INFINITE(group_carrier H)
+        ==> G isomorphic_group H`,
+  REPEAT STRIP_TAC THEN TRANS_TAC ISOMORPHIC_GROUP_TRANS `integer_group` THEN
+  GEN_REWRITE_TAC RAND_CONV [ISOMORPHIC_GROUP_SYM] THEN
+  ASM_SIMP_TAC[ISOMORPHIC_GROUP_INFINITE_CYCLIC_INTEGER]);;
+
+(* ------------------------------------------------------------------------- *)
+(* Free Abelian groups on a set, using the "frag" type constructor.          *)
+(* ------------------------------------------------------------------------- *)
+
+let free_abelian_group = new_definition
+ `free_abelian_group (s:A->bool) =
+    group({c | frag_support c SUBSET s},frag_0,frag_neg,frag_add)`;;
+
+let FREE_ABELIAN_GROUP = prove
+ (`(!s:A->bool.
+        group_carrier(free_abelian_group s) = {c | frag_support c SUBSET s}) /\
+   (!s:A->bool. group_id(free_abelian_group s) = frag_0) /\
+   (!s:A->bool. group_inv(free_abelian_group s) = frag_neg) /\
+   (!s:A->bool. group_mul(free_abelian_group s) = frag_add)`,
+  REWRITE_TAC[AND_FORALL_THM] THEN GEN_TAC THEN
+  MP_TAC(fst(EQ_IMP_RULE
+   (ISPEC(rand(rand(snd(strip_forall(concl free_abelian_group)))))
+   (CONJUNCT2 group_tybij)))) THEN
+  REWRITE_TAC[GSYM free_abelian_group] THEN ANTS_TAC THENL
+   [SIMP_TAC[IN_ELIM_THM; FRAG_SUPPORT_NEG; FRAG_SUPPORT_0; EMPTY_SUBSET] THEN
+    CONJ_TAC THENL
+     [REPEAT STRIP_TAC THEN
+      W(MP_TAC o PART_MATCH lhand FRAG_SUPPORT_ADD o lhand o snd) THEN
+      ASM SET_TAC[];
+      REPEAT STRIP_TAC THEN CONV_TAC FRAG_MODULE];
+    SIMP_TAC[group_carrier; group_id; group_inv; group_mul]]);;
+
+let ABELIAN_FREE_ABELIAN_GROUP = prove
+ (`!s:A->bool. abelian_group(free_abelian_group s)`,
+  REWRITE_TAC[abelian_group; FREE_ABELIAN_GROUP] THEN
+  REPEAT STRIP_TAC THEN CONV_TAC FRAG_MODULE);;
